tests/case-studies/SAT.v
@@ -1,0 +1,321 @@
+From Coq Require Export List.
+From Coq Require Import Nat Recdef Lia.
+Export ListNotations.
+
+(* Verification of a simple SAT solver
+ * -----------------------------------
+ *)
+
+
+(* Types defining the problem and solution
+   ---------------------------------------
+
+   The solver takes as input a query in CNF form, representing a conjunction of
+   clauses, where each clause represents a conjunction of literals.
+
+   Each literal represents a boolean variable (or its negation), and the goal of
+   the solver is to produce a boolean assignation for each literal present in
+   the input formula.
+*)
+
+(* A literal. [Pos n] corresponds to literal n, and [Neg n] to its negation.
+*)
+Inductive literal :=
+  | Pos : nat -> literal
+  | Neg : nat -> literal.
+
+(* A clause represents a disjunction of literals *)
+Definition clause := list literal.
+
+(* A SAT problem in Conjunctive Normal Form:
+   it corresponds to a conjunction of clauses *)
+Definition cnf := list clause.
+
+(* Example:
+
+   The following cnf:
+   [[Pos 1; Neg 2];
+    [Neg 1; Pos 3; Pos 4]]
+
+   corresponds to the boolean formula:
+   (x1 \/ ~x2) /\
+   (~x1 \/ x3 \/ x4)
+
+   where x1, x2, x3 and x4 are boolean variables.
+*)
+
+(* The goal of the solver is to produce an assignment. We represent it as a list
+   of literals, which correspond to the literals that are taken to be true.
+
+   In other words, if the assignment list contains [Neg 3], then the boolean
+   variable x3 should be assigned to false.
+
+   Note: we generally only want to consider "valid" assignments, which do not
+   include both a literal and its negation. We will come back to this later (see
+   [valid_assignment]).
+*)
+Definition assignment := list literal.
+
+(* In fact, the solver we implement will return a list of all possible
+   solutions.
+
+   (This would be terribly inefficient if we were to run the solver and compute
+   the full list of solutions, but we can instead compute it using a
+   call-by-name strategy (thus, the list of solutions becomes a lazy list), and
+   only retrieve the first solution of the list.)
+*)
+Definition solutions := list assignment.
+
+
+(* Helper functions and lemmas
+   ---------------------------
+
+   Mainly define the (computable) equality function on literals,
+   literal negation, and associated lemmas.
+*)
+
+(* Some auxiliary functions on literals. *)
+Definition lit_eqb (l1 l2: literal): bool :=
+  match l1, l2 with
+  | Pos u, Pos v
+  | Neg u, Neg v => u =? v
+  | _, _ => false
+  end.
+
+Lemma lit_eqb_eq l1 l2: lit_eqb l1 l2 = true <-> l1 = l2.
+Proof.
+  destruct l1, l2; cbn; try now (split; congruence).
+  all: rewrite PeanoNat.Nat.eqb_eq; split; congruence.
+Qed.
+
+Lemma lit_eqb_neq l1 l2 : lit_eqb l1 l2 = false <-> l1 <> l2.
+Proof.
+  destruct l1, l2; cbn; try now (split; congruence).
+  all: rewrite PeanoNat.Nat.eqb_neq; split; congruence.
+Qed.
+
+Definition lit_neg (l: literal): literal :=
+  match l with
+  | Pos n => Neg n
+  | Neg n => Pos n
+  end.
+
+Lemma lit_neg_idemp (l: literal) : lit_neg (lit_neg l) = l.
+Proof. destruct l; auto. Qed.
+
+(* The size of a CNF, defined as the the number of its literals.
+   Used to prove termination of the solver. *)
+Fixpoint cnf_size (c: cnf): nat :=
+  match c with
+  | [] => 0
+  | cl :: rest => length cl + cnf_size rest
+  end.
+
+Ltac case_if :=
+  match goal with
+    |- context [if ?b then _ else _] =>
+    destruct b eqn:?
+  end.
+
+Lemma existsb_lit_notin l c : existsb (lit_eqb l) c = false <-> ~ In l c.
+Proof.
+  split.
+  { intros ? ?. enough (existsb (lit_eqb l) c = true) by congruence.
+    apply existsb_exists. eexists; split; eauto. apply lit_eqb_eq; auto. }
+  { intros HH. destruct (existsb (lit_eqb l) c) eqn:Heq; auto. exfalso.
+    apply existsb_exists in Heq as [? [? ->%lit_eqb_eq]]. apply HH. auto. }
+Qed.
+
+
+
+(* The solver definition
+   ------------------------
+
+   This is the implementation of the SAT solver itself.
+
+   Its main function is [resolve]. It relies on the [propagate] auxiliary
+   function, which implements literal propagation.
+
+   The high-level intuition is that [propagate l c] takes a literal [l] and a
+   cnf [c], and, assuming that [l] is to be assigned to true, simplifies [c]
+   into a new cnf which does not rely on [l] or [lit_neg l] anymore.
+
+
+   The [_variant] lemmas can be ignored, they are only used in the (included)
+   proof of termination for defining [resolve].
+*)
+
+Definition remove_lit (l: literal) (cl: clause) :=
+  List.filter (fun l' => negb (lit_eqb l l')) cl.
+
+Fixpoint propagate (l: literal) (c: cnf) : cnf :=
+  match c with
+  | [] => []
+  | cl :: rest =>
+    if List.existsb (lit_eqb l) cl
+    then propagate l rest
+    else (remove_lit (lit_neg l) cl) :: (propagate l rest)
+  end.
+
+Lemma remove_lit_variant (l: literal) (cl: clause):
+  length (remove_lit l cl) <= length cl.
+Proof.
+  induction cl as [| ? ? IHcl]; cbn; try case_if; cbn; auto.
+  unfold remove_lit in IHcl. lia.
+Qed.
+
+Lemma propagate_variant (l: literal) (c: cnf):
+  cnf_size (propagate l c) <= cnf_size c.
+Proof.
+  induction c as [| cl c IHc]; cbn; auto.
+  case_if; cbn; try lia. pose proof (remove_lit_variant (lit_neg l) cl).
+  lia.
+Qed.
+
+Function resolve (c: cnf) {measure cnf_size c}: solutions :=
+  match c with
+  | [] => [[]]
+  | cl :: rest =>
+    match cl with
+    | [] => []
+    | l :: cl' =>
+      let c1 := propagate l rest in
+      let c2 := propagate (lit_neg l) (cl' :: rest) in
+      let solutions1 := List.map (List.cons l) (resolve c1) in
+      let solutions2 := List.map (List.cons (lit_neg l)) (resolve c2) in
+      solutions1 ++ solutions2
+    end
+  end.
+Proof.
+  (* Proof of termination *)
+  all: intros c cl rest l cl'; intros -> ->; cbn.
+  { destruct (existsb (lit_eqb (lit_neg l))); cbn.
+    - pose proof (propagate_variant (lit_neg l) rest). lia.
+    - pose proof (remove_lit_variant (lit_neg (lit_neg l)) cl').
+      pose proof (propagate_variant (lit_neg l) rest). lia. }
+  { pose proof (propagate_variant l rest). lia. }
+Defined.
+
+(* NB: Function generates an induction principle for [resolve], and a lemma to
+   unfold its body. You will need to use them. *)
+Check resolve_ind.
+Check resolve_equation.
+
+
+(* Interpretation of clauses and cnf
+   ------------------------------------
+
+   Given an assignment, we can "evaluate" a clause/a cnf as a boolean.
+   This is done by the [interp] functions below.
+ *)
+
+Fixpoint interp_clause (cl: clause) (a: assignment): bool :=
+  match cl with
+  | [] => false
+  | l :: cl' => List.existsb (lit_eqb l) a || interp_clause cl' a
+  end.
+
+Fixpoint interp (c: cnf) (a: assignment): bool :=
+  match c with
+  | [] => true
+  | cl :: rest => interp_clause cl a && interp rest a
+  end.
+
+
+
+(* To prove correctness of [resolve] in the unsat case we will need to define
+what a *valid* assignment is, i.e. one that does not contain both a literal and
+its negation. *)
+Definition valid_assignment (a: assignment) :=
+  forall (l: literal),
+    List.In l a ->
+    ~ List.In (lit_neg l) a.
+
+    From Coq Require Import List Nat Recdef Lia.
+    Import ListNotations.
+    
+    
+    (* 1) Correctness of solutions returned by [resolve]
+    -------------------------------------------------
+    
+       A first correctness lemma: assignments produced by [resolve] are correct wrt
+       [interp].
+    *)
+    
+    (* The core of the proof relies on a similar correctness lemma for [propagate]. *)
+    Lemma propagate_correct (a: assignment) (l: literal) (c: cnf) :
+      interp (propagate l c) a = true ->
+      interp c (l :: a) = true.
+    Admitted.
+    
+    Lemma resolve_correct (c: cnf) (a: assignment):
+      List.In a (resolve c) ->
+      interp c a = true.
+    Admitted.
+    
+    
+    
+    (* 2) Correctness of [resolve] in the unsat case
+       ---------------------------------------------
+    
+       If [resolve] returns no solutions (the empty list), then the input CNF should
+       be unsatisfiable.
+    
+       To formally state this property, we first need to define what a *valid*
+       assignment is, i.e. one that does not contain both a literal and its negation.
+    *)
+    
+    (* You will need to formulate a lemma for [propagate], in a similar vein as
+       [propagate_correct].
+    
+       However, there's an extra subtlety here. Think: does the following hold
+       if (lit_neg) is in a?
+    
+         interp (propagate l c) a = false ->
+         interp c (l :: a) = false
+    *)
+    
+    Lemma resolve_unsat_correct (c: cnf):
+      resolve c = [] ->
+      forall a, valid_assignment a -> interp c a = false.
+    Admitted.
+    
+    
+    (* ==== This part is OPTIONAL and it is NOT graded. === *)
+    (* ==== We keep this for the sake of completeness of the specification === *)
+    (* ==== but exclude it from grading to keep the task complexity at bay. === *)
+    
+    (* 3) Validity of assignments produced by [resolve]
+       ------------------------------------------------
+    
+       To complete the proof of the solver, we finally need to prove that it only
+       produces valid assignments. Otherwise, a solver could simply return an
+       assignment containing every literal and its negation, which would be
+       considered as a valid solution according to [interp].
+    
+       The key idea is to prove that, for any literal that appears in an assignment
+       returned by [resolve c], then either the literal or its negation were present
+       in [c].
+    *)
+    
+    (* useful helper lemmas *)
+    Lemma valid_assignment_nil : valid_assignment [].
+    Proof. intros ? ?. cbn in *. auto. Qed.
+    
+    Lemma valid_assignment_cons a l:
+      valid_assignment a ->
+      ~ List.In (lit_neg l) a ->
+      valid_assignment (l :: a).
+    Proof.
+      intros Hv Ha l'. cbn. intros [->|Hl'].
+      { intros HH. apply Ha. destruct HH; auto. exfalso.
+        destruct l'; cbn in *; congruence. }
+      { intros [?|HH].
+        { subst l. rewrite lit_neg_idemp in Ha. auto. }
+        { eapply (Hv l' Hl'); auto. } }
+    Qed.
+    
+    Lemma resolve_valid (c: cnf) (a: assignment):
+      List.In a (resolve c) ->
+      valid_assignment a.
+    Admitted.
