tests/case-studies/vfa/SearchTree.v
@@ -1,0 +1,1805 @@
+
+(** * SearchTree: Binary Search Trees *)
+(* Due to VFA's exercise on binary search trees: 
+  https://softwarefoundations.cis.upenn.edu/vfa-current/SearchTree.html
+*)
+
+Require Import MirrorSolve.FirstOrder.
+
+Require Import MirrorSolve.BV.
+Require Import MirrorSolve.SMT.
+Require Import MirrorSolve.UF.
+
+Require Import MirrorSolve.FOLTrees.
+
+Require Import MirrorSolve.HLists.
+Require Import Coq.Lists.List.
+
+Import HListNotations.
+Import ListNotations.
+
+Require Import Coq.Strings.String.
+
+Require Import Coq.ZArith.BinInt.
+Import HListNotations.
+
+Require Import MirrorSolve.BV.
+Require Import MirrorSolve.SMT.
+Require Import MirrorSolve.UF.
+
+Require Import MirrorSolve.Reflection.Core.
+Require Import MirrorSolve.Reflection.FM.
+Require Import MirrorSolve.Reflection.Tactics.
+From Hammer Require Import Hammer.
+
+Set Hammer ATPLimit 5.
+Set Hammer ReconstrLimit 10.
+
+Section Trees.
+  (* type of values in the tree *)
+  Variable (V: Type).
+  Set Universe Polymorphism.
+
+  (*** MS BEGIN {"type": "configuration", "config_type":"boilerplate"} *)
+  
+  Notation sig := FOLTrees.sig.
+  
+  Definition tree_model := FOLTrees.fm_model V.
+
+  MetaCoq Quote Definition t_ite := @ite.
+  MetaCoq Quote Definition t_zlt := @Z.ltb.
+  MetaCoq Quote Definition t_glt := @Z.gtb.
+  MetaCoq Quote Definition t_zlt' := @Z.lt.
+  MetaCoq Quote Definition t_glt' := @Z.gt.
+  MetaCoq Quote Definition t_emp := @Emp.
+  MetaCoq Quote Definition t_node := @Node.
+  MetaCoq Quote Definition t_insert := (@FOLTrees.insert V).
+  MetaCoq Quote Definition t_lookup := (@FOLTrees.lookup V).
+  MetaCoq Quote Definition t_bound := (@FOLTrees.bound V).
+  MetaCoq Quote Definition t_lt_t := (@FOLTrees.lt_t V).
+  MetaCoq Quote Definition t_gt_t := (@FOLTrees.gt_t V).
+  MetaCoq Quote Definition t_ordered := (@FOLTrees.ordered V).
+  
+  Definition is_emp t := eq_ctor t t_emp.
+  Definition is_node t := eq_ctor t t_node.
+  Definition is_zlt t := eq_term t t_zlt.
+  Definition is_zgt t := eq_term t t_glt.
+  Definition is_insert t := eq_ctor t t_insert.
+  Definition is_lookup t := eq_ctor t t_lookup.
+  Definition is_bound t := eq_ctor t t_bound.
+  Definition is_lt_t t := eq_ctor t t_lt_t.
+  Definition is_gt_t t := eq_ctor t t_gt_t.
+  Definition is_ordered t := eq_ctor t t_ordered.
+  Definition is_zlt' t := eq_term t t_zlt'.
+  Definition is_zgt' t := eq_term t t_glt'.
+
+  MetaCoq Quote Definition t_bool := (bool).
+  MetaCoq Quote Definition t_Z := (Z).
+  MetaCoq Quote Definition t_tree := (@tree V).
+  MetaCoq Quote Definition t_V := (V).
+
+  Definition is_cond_b t :=
+    match t with 
+    | tApp f (t :: _) => 
+      andb (eq_term f t_ite) (eq_term t t_bool)
+    | _ => false
+    end.
+
+  Definition is_cond_t t :=
+    match t with 
+    | tApp f (t :: _) => 
+      andb (eq_term f t_ite) (eq_term t t_V)
+    | _ => false
+    end.
+
+  Definition is_cond_tree t :=
+    match t with 
+    | tApp f (t :: _) => 
+      andb (eq_term f t_ite) (eq_term t t_tree)
+    | _ => false
+    end.
+
+  Notation tac_bool := (tacLit sig tree_model bool_lit (fun b => (BS; b)) (fun b _ => (BS; TFun sig (b_lit b) hnil))).
+  Notation tac_fun f := (tacFun _ _ (Mk_fun_sym sig _ _ f)).
+  Notation tac_rel f := (tacRel _ _ (Mk_rel_sym sig _ f)).
+
+  Definition match_tacs : list ((term -> bool) * tac_syn sig tree_model) := [
+      ( is_emp, tac_fun e_f)
+    ; ( is_node, tac_fun t_f)
+    ; ( is_zlt, tac_fun z_lt)
+    ; ( is_zgt, tac_fun z_gt)
+    ; ( is_cond_b, tac_fun cond_b)
+    ; ( is_cond_t, tac_fun cond_t)
+    ; ( is_cond_tree, tac_fun cond_tree)
+    ; ( is_bool_term, tac_bool )
+    ; ( is_lookup, tac_fun lookup_f)
+    ; ( is_bound, tac_fun bound_f)
+    ; ( is_insert, tac_fun insert_f)
+    ; ( is_lt_t, tac_rel lt_t_r)
+    ; ( is_gt_t, tac_rel gt_t_r)
+    ; ( is_ordered, tac_rel ordered_r) 
+    ; ( is_zlt', tac_rel lt_z)
+    ; ( is_zgt', tac_rel gt_z)
+  ].
+
+  Definition match_inds : list ((term -> bool) * FOLTrees.sorts) := [
+      (eq_term t_tree, TreeS)
+    ; (eq_term t_V, TS)
+    ; (eq_term t_bool, BS)
+    ; (eq_term t_Z, ZS)
+  ].
+
+  Local Declare ML Module "mirrorsolve".
+  (*** MS END {"type": "configuration", "config_type":"boilerplate"} *)
+  (*** MS BEGIN {"type": "configuration", "config_type":"plugin"} *)
+  RegisterCustomSort TS "A".
+  (*** MS END {"type": "configuration", "config_type":"plugin"} *)
+
+  (*** MS BEGIN {"type": "configuration", "config_type":"boilerplate"} *)
+  RegisterSMTInd TreeS (SICases [
+    ("node"%string, [SIRec; SISort (SInt tt); SISort (SCustom "A"); SIRec]); 
+    ("emp"%string, [])
+    ]) "A_tree".
+  (*** MS END {"type": "configuration", "config_type":"boilerplate"} *)
+
+  (*** MS BEGIN {"type": "configuration", "config_type":"plugin"} *)
+
+  RegisterSMTSort ZS SInt.
+  RegisterSMTSort BS SBool.
+
+  RegisterSMTUF "bound" BS ZS TreeS.
+  RegisterSMTUF "lookup" TS TS ZS TreeS.
+  RegisterSMTUF "insert" TreeS ZS TS TreeS.
+  RegisterSMTUF "lt_t" BS ZS TreeS.
+  RegisterSMTUF "gt_t" BS ZS TreeS.
+  RegisterSMTUF "ordered" BS TreeS.
+
+  RegisterSMTFun FOLTrees.z_lt "<" 2.
+  RegisterSMTFun FOLTrees.z_gt ">" 2.
+  RegisterSMTFun FOLTrees.lt_z "<" 2.
+  RegisterSMTFun FOLTrees.gt_z ">" 2.
+  RegisterSMTFun FOLTrees.e_f "emp" 0.
+  RegisterSMTFun FOLTrees.t_f "node" 4.
+  RegisterSMTFun FOLTrees.bound_f "bound" 2.
+  RegisterSMTFun FOLTrees.lookup_f "lookup" 3.
+  RegisterSMTFun FOLTrees.insert_f "insert" 3.
+  RegisterSMTFun FOLTrees.lt_t_r "lt_t" 2.
+  RegisterSMTFun FOLTrees.gt_t_r "gt_t" 2.
+  RegisterSMTFun FOLTrees.ordered_r "ordered" 1.
+  RegisterSMTFun FOLTrees.cond_b "ite" 3.
+  RegisterSMTFun FOLTrees.cond_t "ite" 3.
+  RegisterSMTFun FOLTrees.cond_tree "ite" 3.
+
+  RegisterSMTBuiltin FOLTrees.b_lit BoolLit.
+  (*** MS END {"type": "configuration", "config_type":"plugin"} *)
+
+  (*** MS BEGIN {"type": "configuration", "config_type":"boilerplate"} *)
+  Transparent denote_tm.
+  Require Import MirrorSolve.Axioms.
+
+  Ltac check_goal_unsat := 
+    match goal with 
+    | |- ?G => check_unsat_neg G; eapply UnsoundAxioms.interp_true
+    end.
+
+  (*** MS END {"type": "configuration", "config_type":"boilerplate"} *)
+  (*** MS BEGIN {"type": "configuration", "config_type":"tactics"} *)
+  Ltac pose_lookup_axioms := Utils.pose_all (tt, @lookup_emp V, @lookup_node V).
+  Ltac pose_bound_axioms := Utils.pose_all (tt, @bound_emp V, @bound_node V).
+  Ltac pose_insert_axioms := Utils.pose_all (tt, @insert_emp V, @insert_node V).
+  Ltac pose_ordered_axioms := Utils.pose_all (tt, @lt_t_emp V, @lt_t_node V, @gt_t_emp V, @gt_t_node V, @ordered_emp V, @ordered_node V).
+
+  Ltac pose_tree_axioms := pose_lookup_axioms; 
+    pose_bound_axioms; 
+    pose_insert_axioms; 
+    pose_ordered_axioms.
+
+  Ltac prep_proof := pose_tree_axioms; 
+    Utils.revert_all; 
+    unfold "<->" in *;
+    intros V.
+
+  Ltac reflect t := reflect_goal_trust FOLTrees.sig tree_model FOLTrees.sorts_eq_dec match_tacs match_inds t.
+  (*** MS END {"type": "configuration", "config_type":"tactics"} *)
+
+  (*** MS BEGIN {"type": "configuration", "config_type":"boilerplate"} *)
+  MetaCoq Quote Definition lookup_empty_goal := (
+    (forall (d : V) (x : Z) (l : tree V) (y : Z) (v : V) (r : tree V),
+ lookup d x (Node l y v r) = ite (x <? y)%Z (lookup d x l) (ite (x >? y)%Z (lookup d x r) v)) ->
+(forall (d : V) (x : Z), lookup d x Emp = d) ->
+(forall (x : Z) (l : tree V) (y : Z) (v : V) (r : tree V),
+ bound x (Node l y v r) = ite (x <? y)%Z (bound x l) (ite (x >? y)%Z (bound x r) true)) ->
+(forall x : Z, bound x Emp = false) ->
+(forall (x : Z) (v : V) (l : tree V) (y : Z) (v' : V) (r : tree V),
+ insert x v (Node l y v' r) =
+ ite (x <? y)%Z (Node (insert x v l) y v' r)
+   (ite (x >? y)%Z (Node l y v' (insert x v r)) (Node l x v r))) ->
+(forall (x : Z) (v : V), insert x v Emp = Node Emp x v Emp) ->
+(forall (l : tree V) (k : Z) (v : V) (r : tree V),
+ (lt_t k l /\ gt_t k r /\ ordered l /\ ordered r -> ordered (Node l k v r)) /\
+ (ordered (Node l k v r) -> lt_t k l /\ gt_t k r /\ ordered l /\ ordered r)) ->
+ordered Emp ->
+(forall (k : Z) (l : tree V) (k' : Z) (v : V) (r : tree V),
+ ((k' > k)%Z /\ gt_t k l /\ gt_t k r -> gt_t k (Node l k' v r)) /\
+ (gt_t k (Node l k' v r) -> (k' > k)%Z /\ gt_t k l /\ gt_t k r)) ->
+(forall k : Z, gt_t k Emp) ->
+(forall (k : Z) (l : tree V) (k' : Z) (v : V) (r : tree V),
+ ((k' < k)%Z /\ lt_t k l /\ lt_t k r -> lt_t k (Node l k' v r)) /\
+ (lt_t k (Node l k' v r) -> (k' < k)%Z /\ lt_t k l /\ lt_t k r)) ->
+(forall k : Z, lt_t k Emp) -> forall (d : V) (k : Z), lookup d k Emp = d
+  ).
+  (*** MS END {"type": "configuration", "config_type":"boilerplate"} *)
+
+  (* hammer handles this one (it's easy) *)
+  (*** MS BEGIN {"type": "configuration", "config_type":"plugin"} *)
+  SetSMTSolver "cvc5".
+  (*** MS END {"type": "configuration", "config_type":"plugin"} *)
+  (*** MS BEGIN {"type": "proof_definition"} *)
+  Theorem lookup_empty : 
+    forall (d: V) (k : Z),
+      lookup d k Emp = d.
+  (*** MS END {"type": "proof_definition"} *)
+  Proof.
+    (*** MS BEGIN {"type": "proof", "proof_type":"manual"} *)
+    intros.
+    trivial.
+    (*** MS END {"type": "proof", "proof_type":"manual"} *)
+    Restart.
+  Proof.
+    (*** MS BEGIN {"type": "proof", "proof_type":"hammer", "total":1, "finished":1} *)
+    hammer.
+    (*** MS END {"type": "proof", "proof_type":"hammer", "total":1, "finished":1} *)
+  Restart.
+  Proof.
+    (*** MS BEGIN {"type": "proof", "proof_type":"mirrorsolve", "total":1} *)
+    prep_proof.
+    reflect lookup_empty_goal; 
+    check_goal_unsat.
+    (*** MS END {"type": "proof", "proof_type":"mirrorsolve", "total":1} *)
+  Admitted. (* some weird evaluation issue, can't QED... *)
+
+  (*** MS BEGIN {"type": "configuration", "config_type":"boilerplate"} *)
+  MetaCoq Quote Definition lookup_insert_emp := (
+    
+(forall (d : V) (x : Z) (l : tree V) (y : Z) (v : V) (r : tree V),
+lookup d x (Node l y v r) = ite (x <? y)%Z (lookup d x l) (ite (x >? y)%Z (lookup d x r) v)) ->
+(forall (d : V) (x : Z), lookup d x Emp = d) ->
+(forall (x : Z) (l : tree V) (y : Z) (v : V) (r : tree V),
+bound x (Node l y v r) = ite (x <? y)%Z (bound x l) (ite (x >? y)%Z (bound x r) true)) ->
+(forall x : Z, bound x Emp = false) ->
+(forall (x : Z) (v : V) (l : tree V) (y : Z) (v' : V) (r : tree V),
+insert x v (Node l y v' r) =
+ite (x <? y)%Z (Node (insert x v l) y v' r) (ite (x >? y)%Z (Node l y v' (insert x v r)) (Node l x v r))) ->
+(forall (x : Z) (v : V), insert x v Emp = Node Emp x v Emp) ->
+(forall (l : tree V) (k : Z) (v : V) (r : tree V),
+(lt_t k l /\ gt_t k r /\ ordered l /\ ordered r -> ordered (Node l k v r)) /\
+(ordered (Node l k v r) -> lt_t k l /\ gt_t k r /\ ordered l /\ ordered r)) ->
+ordered Emp ->
+(forall (k : Z) (l : tree V) (k' : Z) (v : V) (r : tree V),
+((k' > k)%Z /\ gt_t k l /\ gt_t k r -> gt_t k (Node l k' v r)) /\
+(gt_t k (Node l k' v r) -> (k' > k)%Z /\ gt_t k l /\ gt_t k r)) ->
+(forall k : Z, gt_t k Emp) ->
+(forall (k : Z) (l : tree V) (k' : Z) (v : V) (r : tree V),
+((k' < k)%Z /\ lt_t k l /\ lt_t k r -> lt_t k (Node l k' v r)) /\
+(lt_t k (Node l k' v r) -> (k' < k)%Z /\ lt_t k l /\ lt_t k r)) ->
+(forall k : Z, lt_t k Emp) ->
+forall (d : V) (k k' : Z) (v : V), k = k' -> lookup d k (insert k' v Emp) = v
+).
+
+  MetaCoq Quote Definition lookup_insert_node := (
+    forall (t1 : tree V) (k : Z) (v : V) (t2 : tree V),
+(forall (d : V) (k0 k' : Z) (v0 : V), k0 = k' -> lookup d k0 (insert k' v0 t1) = v0) ->
+(forall (d : V) (k0 k' : Z) (v0 : V), k0 = k' -> lookup d k0 (insert k' v0 t2) = v0) ->
+(forall (d : V) (x : Z) (l : tree V) (y : Z) (v0 : V) (r : tree V),
+ lookup d x (Node l y v0 r) = ite (x <? y)%Z (lookup d x l) (ite (x >? y)%Z (lookup d x r) v0)) ->
+(forall (d : V) (x : Z), lookup d x Emp = d) ->
+(forall (x : Z) (l : tree V) (y : Z) (v0 : V) (r : tree V),
+ bound x (Node l y v0 r) = ite (x <? y)%Z (bound x l) (ite (x >? y)%Z (bound x r) true)) ->
+(forall x : Z, bound x Emp = false) ->
+(forall (x : Z) (v0 : V) (l : tree V) (y : Z) (v' : V) (r : tree V),
+ insert x v0 (Node l y v' r) =
+ ite (x <? y)%Z (Node (insert x v0 l) y v' r)
+   (ite (x >? y)%Z (Node l y v' (insert x v0 r)) (Node l x v0 r))) ->
+(forall (x : Z) (v0 : V), insert x v0 Emp = Node Emp x v0 Emp) ->
+(forall (l : tree V) (k0 : Z) (v0 : V) (r : tree V),
+ (lt_t k0 l /\ gt_t k0 r /\ ordered l /\ ordered r -> ordered (Node l k0 v0 r)) /\
+ (ordered (Node l k0 v0 r) -> lt_t k0 l /\ gt_t k0 r /\ ordered l /\ ordered r)) ->
+ordered Emp ->
+(forall (k0 : Z) (l : tree V) (k' : Z) (v0 : V) (r : tree V),
+ ((k' > k0)%Z /\ gt_t k0 l /\ gt_t k0 r -> gt_t k0 (Node l k' v0 r)) /\
+ (gt_t k0 (Node l k' v0 r) -> (k' > k0)%Z /\ gt_t k0 l /\ gt_t k0 r)) ->
+(forall k0 : Z, gt_t k0 Emp) ->
+(forall (k0 : Z) (l : tree V) (k' : Z) (v0 : V) (r : tree V),
+ ((k' < k0)%Z /\ lt_t k0 l /\ lt_t k0 r -> lt_t k0 (Node l k' v0 r)) /\
+ (lt_t k0 (Node l k' v0 r) -> (k' < k0)%Z /\ lt_t k0 l /\ lt_t k0 r)) ->
+(forall k0 : Z, lt_t k0 Emp) ->
+forall (d : V) (k0 k' : Z) (v0 : V), k0 = k' -> lookup d k0 (insert k' v0 (Node t1 k v t2)) = v0
+  ).
+  (*** MS END {"type": "configuration", "config_type":"boilerplate"} *)
+
+
+  (*** MS BEGIN {"type": "proof_definition"} *)
+  Theorem lookup_insert_eq : 
+    forall (t : tree V) d k k' v,
+      k = k' ->
+      lookup d k (insert k' v t)  = v.
+  (*** MS END {"type": "proof_definition"} *)
+  Proof.
+    (*** MS BEGIN {"type": "proof", "proof_type":"manual"} *)
+    induction t;
+    intros;
+    simpl in *;
+    subst.
+    - destruct (_ <? _)%Z eqn:?;
+      simpl in *; [
+          Lia.lia
+        |
+      ].
+      destruct (_ >? _)%Z eqn:?;
+      simpl in *; [
+          Lia.lia
+        | trivial
+      ].
+    - destruct (_ <? _)%Z eqn:?;
+      simpl in *.
+      * erewrite Heqb;
+        simpl;
+        eapply IHt1;
+        trivial.
+      * destruct (_ >? _)%Z eqn:?;
+        try erewrite Heqb0;
+        simpl in *;
+        try erewrite Heqb;
+        simpl;
+        try erewrite Heqb0;
+        simpl.
+        + eapply IHt2.
+          trivial.
+        + destruct (k' <? k')%Z eqn:?;
+          simpl; [
+              Lia.lia
+            |
+          ].
+          destruct (k' >? k')%Z eqn:?;
+          simpl; [
+              Lia.lia
+            | trivial
+          ]. 
+    (*** MS END {"type": "proof", "proof_type":"manual"} *)
+  Restart.
+  Proof.
+    (*** MS BEGIN {"type": "proof", "proof_type":"hammer", "total":2, "finished":0} *)
+    induction t.
+    (* - try hammer; admit.   
+    - try hammer; admit. *)
+    (*** MS END {"type": "proof", "proof_type":"hammer", "total":2, "finished":0} *)
+    Restart.
+  Proof.
+    induction t; 
+    prep_proof.
+    - reflect lookup_insert_emp; 
+      check_goal_unsat.
+    - reflect lookup_insert_node; 
+      check_goal_unsat.
+  Admitted.
+
+(*** MS BEGIN {"type": "configuration", "config_type":"boilerplate"} *)
+  MetaCoq Quote Definition lookup_insert_neq_emp := (
+    (forall (d : V) (x : Z) (l : tree V) (y : Z) (v : V) (r : tree V),
+ lookup d x (Node l y v r) =
+ ite (x <? y)%Z (lookup d x l) (ite (x >? y)%Z (lookup d x r) v)) ->
+(forall (d : V) (x : Z), lookup d x Emp = d) ->
+(forall (x : Z) (l : tree V) (y : Z) (v : V) (r : tree V),
+ bound x (Node l y v r) = ite (x <? y)%Z (bound x l) (ite (x >? y)%Z (bound x r) true)) ->
+(forall x : Z, bound x Emp = false) ->
+(forall (x : Z) (v : V) (l : tree V) (y : Z) (v' : V) (r : tree V),
+ insert x v (Node l y v' r) =
+ ite (x <? y)%Z (Node (insert x v l) y v' r)
+   (ite (x >? y)%Z (Node l y v' (insert x v r)) (Node l x v r))) ->
+(forall (x : Z) (v : V), insert x v Emp = Node Emp x v Emp) ->
+(forall (l : tree V) (k : Z) (v : V) (r : tree V),
+ (lt_t k l /\ gt_t k r /\ ordered l /\ ordered r -> ordered (Node l k v r)) /\
+ (ordered (Node l k v r) -> lt_t k l /\ gt_t k r /\ ordered l /\ ordered r)) ->
+ordered Emp ->
+(forall (k : Z) (l : tree V) (k' : Z) (v : V) (r : tree V),
+ ((k' > k)%Z /\ gt_t k l /\ gt_t k r -> gt_t k (Node l k' v r)) /\
+ (gt_t k (Node l k' v r) -> (k' > k)%Z /\ gt_t k l /\ gt_t k r)) ->
+(forall k : Z, gt_t k Emp) ->
+(forall (k : Z) (l : tree V) (k' : Z) (v : V) (r : tree V),
+ ((k' < k)%Z /\ lt_t k l /\ lt_t k r -> lt_t k (Node l k' v r)) /\
+ (lt_t k (Node l k' v r) -> (k' < k)%Z /\ lt_t k l /\ lt_t k r)) ->
+(forall k : Z, lt_t k Emp) ->
+forall (d : V) (k k' : Z) (v : V),
+k <> k' -> lookup d k' (insert k v Emp) = lookup d k' Emp
+).
+
+  MetaCoq Quote Definition lookup_insert_neq_node := (
+    forall (t1 : tree V) (k : Z) (v : V) (t2 : tree V),
+(forall (d : V) (k0 k' : Z) (v0 : V),
+ k0 <> k' -> lookup d k' (insert k0 v0 t1) = lookup d k' t1) ->
+(forall (d : V) (k0 k' : Z) (v0 : V),
+ k0 <> k' -> lookup d k' (insert k0 v0 t2) = lookup d k' t2) ->
+(forall (d : V) (x : Z) (l : tree V) (y : Z) (v0 : V) (r : tree V),
+ lookup d x (Node l y v0 r) =
+ ite (x <? y)%Z (lookup d x l) (ite (x >? y)%Z (lookup d x r) v0)) ->
+(forall (d : V) (x : Z), lookup d x Emp = d) ->
+(forall (x : Z) (l : tree V) (y : Z) (v0 : V) (r : tree V),
+ bound x (Node l y v0 r) = ite (x <? y)%Z (bound x l) (ite (x >? y)%Z (bound x r) true)) ->
+(forall x : Z, bound x Emp = false) ->
+(forall (x : Z) (v0 : V) (l : tree V) (y : Z) (v' : V) (r : tree V),
+ insert x v0 (Node l y v' r) =
+ ite (x <? y)%Z (Node (insert x v0 l) y v' r)
+   (ite (x >? y)%Z (Node l y v' (insert x v0 r)) (Node l x v0 r))) ->
+(forall (x : Z) (v0 : V), insert x v0 Emp = Node Emp x v0 Emp) ->
+(forall (l : tree V) (k0 : Z) (v0 : V) (r : tree V),
+ (lt_t k0 l /\ gt_t k0 r /\ ordered l /\ ordered r -> ordered (Node l k0 v0 r)) /\
+ (ordered (Node l k0 v0 r) -> lt_t k0 l /\ gt_t k0 r /\ ordered l /\ ordered r)) ->
+ordered Emp ->
+(forall (k0 : Z) (l : tree V) (k' : Z) (v0 : V) (r : tree V),
+ ((k' > k0)%Z /\ gt_t k0 l /\ gt_t k0 r -> gt_t k0 (Node l k' v0 r)) /\
+ (gt_t k0 (Node l k' v0 r) -> (k' > k0)%Z /\ gt_t k0 l /\ gt_t k0 r)) ->
+(forall k0 : Z, gt_t k0 Emp) ->
+(forall (k0 : Z) (l : tree V) (k' : Z) (v0 : V) (r : tree V),
+ ((k' < k0)%Z /\ lt_t k0 l /\ lt_t k0 r -> lt_t k0 (Node l k' v0 r)) /\
+ (lt_t k0 (Node l k' v0 r) -> (k' < k0)%Z /\ lt_t k0 l /\ lt_t k0 r)) ->
+(forall k0 : Z, lt_t k0 Emp) ->
+forall (d : V) (k0 k' : Z) (v0 : V),
+k0 <> k' -> lookup d k' (insert k0 v0 (Node t1 k v t2)) = lookup d k' (Node t1 k v t2) 
+).
+  (*** MS END {"type": "configuration", "config_type":"boilerplate"} *)
+
+
+  (* hammer does not handle this one *)
+  (*** MS BEGIN {"type": "proof_definition"} *)
+  Theorem lookup_insert_neq :
+    forall (t: tree V) d k k' v,
+      k <> k' -> 
+      lookup d k' (insert k v t) = lookup d k' t.
+  (*** MS END {"type": "proof_definition"} *)
+  Proof.
+    (*** MS BEGIN {"type": "proof", "proof_type":"manual"} *)
+    induction t;
+    simpl in *;
+    intros.
+    - destruct (_ <? _)%Z eqn:?;
+      simpl in *; [
+          trivial
+        |
+      ].
+      destruct (_ >? _)%Z eqn:?;
+      simpl in *; [
+          trivial
+        | Lia.lia
+      ].
+    - destruct (_ <? _)%Z eqn:?;
+      simpl in *.
+      * erewrite IHt1;
+        trivial.
+      * destruct (_ >? _)%Z eqn:?;
+        simpl.
+        + erewrite IHt2;
+          trivial.
+        + assert (k0 = k) by Lia.lia.
+          subst.
+          destruct (k' <? k)%Z eqn:?; 
+          simpl in *; [
+              trivial
+            | 
+          ].
+          destruct (k' >? k)%Z eqn:?; 
+          simpl in *; [
+              trivial
+            | Lia.lia
+          ].
+    (*** MS END {"type": "proof", "proof_type":"manual"} *)
+    Restart.
+  Proof.
+    (*** MS BEGIN {"type": "proof", "proof_type":"hammer", "total":2, "finished":0} *)
+    induction t. 
+    (* - try hammer. admit.
+    - try hammer. admit. *)
+    (*** MS END {"type": "proof", "proof_type":"hammer", "total":2, "finished":0} *)
+    Restart.
+  Proof.
+    (*** MS BEGIN {"type": "proof", "proof_type":"mirrorsolve", "total":2} *)
+    induction t; 
+    prep_proof.
+    - reflect lookup_insert_neq_emp; 
+      check_goal_unsat.
+    - reflect lookup_insert_neq_node; 
+      check_goal_unsat.
+    (*** MS END {"type": "proof", "proof_type":"mirrorsolve", "total":2} *)
+  Admitted.
+
+
+(** **** Exercise: 3 stars, standard, optional (bound_correct) *)
+
+(** Specify and prove the correctness of [bound]. State and prove
+    three theorems, inspired by those we just proved for [lookup]. *)
+
+(* FILL IN HERE *)
+
+(** **** Exercise: 3 stars, standard, optional (bound_default) *)
+
+(** Prove that if [bound] returns [false], then [lookup] returns
+    the default value. Proceed by induction on the tree. *)
+
+(*** MS BEGIN {"type": "configuration", "config_type":"boilerplate"} *)
+    MetaCoq Quote Definition bound_default_emp := (
+      forall (k : Z) (d : V),
+(forall (d0 : V) (x : Z) (l : tree V) (y : Z) (v : V) (r : tree V),
+ lookup d0 x (Node l y v r) = ite (x <? y)%Z (lookup d0 x l) (ite (x >? y)%Z (lookup d0 x r) v)) ->
+(forall (d0 : V) (x : Z), lookup d0 x Emp = d0) ->
+(forall (x : Z) (l : tree V) (y : Z) (v : V) (r : tree V),
+ bound x (Node l y v r) = ite (x <? y)%Z (bound x l) (ite (x >? y)%Z (bound x r) true)) ->
+(forall x : Z, bound x Emp = false) ->
+(forall (x : Z) (v : V) (l : tree V) (y : Z) (v' : V) (r : tree V),
+ insert x v (Node l y v' r) =
+ ite (x <? y)%Z (Node (insert x v l) y v' r) (ite (x >? y)%Z (Node l y v' (insert x v r)) (Node l x v r))) ->
+(forall (x : Z) (v : V), insert x v Emp = Node Emp x v Emp) ->
+(forall (l : tree V) (k0 : Z) (v : V) (r : tree V),
+ (lt_t k0 l /\ gt_t k0 r /\ ordered l /\ ordered r -> ordered (Node l k0 v r)) /\
+ (ordered (Node l k0 v r) -> lt_t k0 l /\ gt_t k0 r /\ ordered l /\ ordered r)) ->
+ordered Emp ->
+(forall (k0 : Z) (l : tree V) (k' : Z) (v : V) (r : tree V),
+ ((k' > k0)%Z /\ gt_t k0 l /\ gt_t k0 r -> gt_t k0 (Node l k' v r)) /\
+ (gt_t k0 (Node l k' v r) -> (k' > k0)%Z /\ gt_t k0 l /\ gt_t k0 r)) ->
+(forall k0 : Z, gt_t k0 Emp) ->
+(forall (k0 : Z) (l : tree V) (k' : Z) (v : V) (r : tree V),
+ ((k' < k0)%Z /\ lt_t k0 l /\ lt_t k0 r -> lt_t k0 (Node l k' v r)) /\
+ (lt_t k0 (Node l k' v r) -> (k' < k0)%Z /\ lt_t k0 l /\ lt_t k0 r)) ->
+(forall k0 : Z, lt_t k0 Emp) -> bound k Emp = false -> lookup d k Emp = d
+    ).
+  
+    MetaCoq Quote Definition bound_default_node := (
+      
+forall (k : Z) (d : V) (t1 : tree V) (k0 : Z) (v : V) (t2 : tree V),
+(bound k t1 = false -> lookup d k t1 = d) ->
+(bound k t2 = false -> lookup d k t2 = d) ->
+(forall (d0 : V) (x : Z) (l : tree V) (y : Z) (v0 : V) (r : tree V),
+ lookup d0 x (Node l y v0 r) = ite (x <? y)%Z (lookup d0 x l) (ite (x >? y)%Z (lookup d0 x r) v0)) ->
+(forall (d0 : V) (x : Z), lookup d0 x Emp = d0) ->
+(forall (x : Z) (l : tree V) (y : Z) (v0 : V) (r : tree V),
+ bound x (Node l y v0 r) = ite (x <? y)%Z (bound x l) (ite (x >? y)%Z (bound x r) true)) ->
+(forall x : Z, bound x Emp = false) ->
+(forall (x : Z) (v0 : V) (l : tree V) (y : Z) (v' : V) (r : tree V),
+ insert x v0 (Node l y v' r) =
+ ite (x <? y)%Z (Node (insert x v0 l) y v' r) (ite (x >? y)%Z (Node l y v' (insert x v0 r)) (Node l x v0 r))) ->
+(forall (x : Z) (v0 : V), insert x v0 Emp = Node Emp x v0 Emp) ->
+(forall (l : tree V) (k1 : Z) (v0 : V) (r : tree V),
+ (lt_t k1 l /\ gt_t k1 r /\ ordered l /\ ordered r -> ordered (Node l k1 v0 r)) /\
+ (ordered (Node l k1 v0 r) -> lt_t k1 l /\ gt_t k1 r /\ ordered l /\ ordered r)) ->
+ordered Emp ->
+(forall (k1 : Z) (l : tree V) (k' : Z) (v0 : V) (r : tree V),
+ ((k' > k1)%Z /\ gt_t k1 l /\ gt_t k1 r -> gt_t k1 (Node l k' v0 r)) /\
+ (gt_t k1 (Node l k' v0 r) -> (k' > k1)%Z /\ gt_t k1 l /\ gt_t k1 r)) ->
+(forall k1 : Z, gt_t k1 Emp) ->
+(forall (k1 : Z) (l : tree V) (k' : Z) (v0 : V) (r : tree V),
+ ((k' < k1)%Z /\ lt_t k1 l /\ lt_t k1 r -> lt_t k1 (Node l k' v0 r)) /\
+ (lt_t k1 (Node l k' v0 r) -> (k' < k1)%Z /\ lt_t k1 l /\ lt_t k1 r)) ->
+(forall k1 : Z, lt_t k1 Emp) -> bound k (Node t1 k0 v t2) = false -> lookup d k (Node t1 k0 v t2) = d
+    ).
+(*** MS END {"type": "configuration", "config_type":"boilerplate"} *)
+
+    (* hammer handles this one *)
+  (*** MS BEGIN {"type": "proof_definition"} *)
+  Theorem bound_default :
+    forall k d (t: tree V),
+      bound k t = false ->
+      lookup d k t = d.
+  (*** MS END {"type": "proof_definition"} *)
+  Proof.
+    (*** MS BEGIN {"type": "proof", "proof_type":"manual"} *)
+    induction t;
+    simpl in *;
+    intros; 
+    trivial.
+    destruct (_ <? _)%Z eqn:?;
+    simpl in *; [
+        intuition eauto
+      |
+    ].
+    destruct (_ >? _)%Z eqn:?;
+    simpl in *; [
+        intuition eauto
+      | congruence
+    ].
+    (*** MS END {"type": "proof", "proof_type":"manual"} *)
+    Restart.
+  Proof.
+    (*** MS BEGIN {"type": "proof", "proof_type":"hammer", "total":2, "finished":1} *)
+    induction t.
+    - try hammer.
+    - admit. (* - try hammer; admit. *)
+    (*** MS END {"type": "proof", "proof_type":"hammer", "total":2, "finished":1} *)
+    Restart.
+    
+  Proof.
+    (*** MS BEGIN {"type": "proof", "proof_type":"mirrorsolve", "total":2} *)
+    induction t; 
+    prep_proof. 
+    - reflect bound_default_emp; 
+      check_goal_unsat.
+    - reflect bound_default_node; 
+      check_goal_unsat.
+    (*** MS END {"type": "proof", "proof_type":"mirrorsolve", "total":2} *)
+  Admitted.
+
+(** [] *)
+
+(* ################################################################# *)
+(** * BSTs vs. Higher-order Functions (Optional) *)
+
+(** The three theorems we just proved for [lookup] should seem
+    familiar: we proved equivalent theorems in [Maps] for maps
+    defined as higher-order functions. *)
+
+(** Let's prove analogues to these three theorems for search trees.
+
+    Hint: you do not need to unfold the definitions of [empty_tree],
+    [insert], or [lookup].  Instead, use [lookup_insert_eq] and
+    [lookup_insert_neq]. *)
+
+(** **** Exercise: 2 stars, standard, optional (lookup_insert_shadow) *)
+
+
+  (*** MS BEGIN {"type": "configuration", "config_type":"boilerplate"} *)
+MetaCoq Quote Definition lookup_insert_shadow_emp := (
+  (forall (d : V) (x : Z) (l : tree V) (y : Z) (v : V) (r : tree V),
+ lookup d x (Node l y v r) = ite (x <? y)%Z (lookup d x l) (ite (x >? y)%Z (lookup d x r) v)) ->
+(forall (d : V) (x : Z), lookup d x Emp = d) ->
+(forall (x : Z) (l : tree V) (y : Z) (v : V) (r : tree V),
+ bound x (Node l y v r) = ite (x <? y)%Z (bound x l) (ite (x >? y)%Z (bound x r) true)) ->
+(forall x : Z, bound x Emp = false) ->
+(forall (x : Z) (v : V) (l : tree V) (y : Z) (v' : V) (r : tree V),
+ insert x v (Node l y v' r) =
+ ite (x <? y)%Z (Node (insert x v l) y v' r) (ite (x >? y)%Z (Node l y v' (insert x v r)) (Node l x v r))) ->
+(forall (x : Z) (v : V), insert x v Emp = Node Emp x v Emp) ->
+(forall (l : tree V) (k : Z) (v : V) (r : tree V),
+ (lt_t k l /\ gt_t k r /\ ordered l /\ ordered r -> ordered (Node l k v r)) /\
+ (ordered (Node l k v r) -> lt_t k l /\ gt_t k r /\ ordered l /\ ordered r)) ->
+ordered Emp ->
+(forall (k : Z) (l : tree V) (k' : Z) (v : V) (r : tree V),
+ ((k' > k)%Z /\ gt_t k l /\ gt_t k r -> gt_t k (Node l k' v r)) /\
+ (gt_t k (Node l k' v r) -> (k' > k)%Z /\ gt_t k l /\ gt_t k r)) ->
+(forall k : Z, gt_t k Emp) ->
+(forall (k : Z) (l : tree V) (k' : Z) (v : V) (r : tree V),
+ ((k' < k)%Z /\ lt_t k l /\ lt_t k r -> lt_t k (Node l k' v r)) /\
+ (lt_t k (Node l k' v r) -> (k' < k)%Z /\ lt_t k l /\ lt_t k r)) ->
+(forall k : Z, lt_t k Emp) ->
+forall (v v' d : V) (k k' : Z), lookup d k' (insert k v (insert k v' Emp)) = lookup d k' (insert k v Emp)
+).
+
+MetaCoq Quote Definition lookup_insert_shadow_node := (
+  
+forall (t1 : tree V) (k : Z) (v : V) (t2 : tree V),
+(forall (v0 v' d : V) (k0 k' : Z), lookup d k' (insert k0 v0 (insert k0 v' t1)) = lookup d k' (insert k0 v0 t1)) ->
+(forall (v0 v' d : V) (k0 k' : Z), lookup d k' (insert k0 v0 (insert k0 v' t2)) = lookup d k' (insert k0 v0 t2)) ->
+(forall (d : V) (x : Z) (l : tree V) (y : Z) (v0 : V) (r : tree V),
+ lookup d x (Node l y v0 r) = ite (x <? y)%Z (lookup d x l) (ite (x >? y)%Z (lookup d x r) v0)) ->
+(forall (d : V) (x : Z), lookup d x Emp = d) ->
+(forall (x : Z) (l : tree V) (y : Z) (v0 : V) (r : tree V),
+ bound x (Node l y v0 r) = ite (x <? y)%Z (bound x l) (ite (x >? y)%Z (bound x r) true)) ->
+(forall x : Z, bound x Emp = false) ->
+(forall (x : Z) (v0 : V) (l : tree V) (y : Z) (v' : V) (r : tree V),
+ insert x v0 (Node l y v' r) =
+ ite (x <? y)%Z (Node (insert x v0 l) y v' r) (ite (x >? y)%Z (Node l y v' (insert x v0 r)) (Node l x v0 r))) ->
+(forall (x : Z) (v0 : V), insert x v0 Emp = Node Emp x v0 Emp) ->
+(forall (l : tree V) (k0 : Z) (v0 : V) (r : tree V),
+ (lt_t k0 l /\ gt_t k0 r /\ ordered l /\ ordered r -> ordered (Node l k0 v0 r)) /\
+ (ordered (Node l k0 v0 r) -> lt_t k0 l /\ gt_t k0 r /\ ordered l /\ ordered r)) ->
+ordered Emp ->
+(forall (k0 : Z) (l : tree V) (k' : Z) (v0 : V) (r : tree V),
+ ((k' > k0)%Z /\ gt_t k0 l /\ gt_t k0 r -> gt_t k0 (Node l k' v0 r)) /\
+ (gt_t k0 (Node l k' v0 r) -> (k' > k0)%Z /\ gt_t k0 l /\ gt_t k0 r)) ->
+(forall k0 : Z, gt_t k0 Emp) ->
+(forall (k0 : Z) (l : tree V) (k' : Z) (v0 : V) (r : tree V),
+ ((k' < k0)%Z /\ lt_t k0 l /\ lt_t k0 r -> lt_t k0 (Node l k' v0 r)) /\
+ (lt_t k0 (Node l k' v0 r) -> (k' < k0)%Z /\ lt_t k0 l /\ lt_t k0 r)) ->
+(forall k0 : Z, lt_t k0 Emp) ->
+forall (v0 v' d : V) (k0 k' : Z),
+lookup d k' (insert k0 v0 (insert k0 v' (Node t1 k v t2))) = lookup d k' (insert k0 v0 (Node t1 k v t2))
+).
+  (*** MS END {"type": "configuration", "config_type":"boilerplate"} *)
+
+  (* hammer does not handle this one *)
+  (*** MS BEGIN {"type": "proof_definition"} *)
+  Lemma lookup_insert_shadow :
+    forall (t: tree V) v v' d k k',
+      lookup d k' (insert k v (insert k v' t)) = lookup d k' (insert k v t).
+  (*** MS END {"type": "proof_definition"} *)
+  Proof.
+    (*** MS BEGIN {"type": "proof", "proof_type":"manual"} *)
+    induction t;
+    simpl in *;
+    intros.
+    - assert ((k <? k)%Z = false) by Lia.lia. 
+      erewrite H;
+      simpl.
+      assert ((k >? k)%Z = false) by Lia.lia. 
+      erewrite H0;
+      simpl.
+      trivial.
+    - destruct (_ <? _)%Z eqn:?;
+      simpl in *.
+      + erewrite Heqb;
+        simpl.
+        f_equal.
+        eapply IHt1.
+      + destruct (_ >? _)%Z eqn:?;
+        simpl in *.
+        * erewrite Heqb.
+          erewrite Heqb0.
+          simpl.
+          f_equal.
+          f_equal.
+          eapply IHt2.
+        * assert ((k0 <? k0)%Z = false) by Lia.lia.
+          assert ((k0 >? k0)%Z = false) by Lia.lia.
+          erewrite H.
+          erewrite H0.
+          simpl.
+          f_equal.
+    (*** MS END {"type": "proof", "proof_type":"manual"} *)
+    Restart.   
+  Proof.
+    (*** MS BEGIN {"type": "proof", "proof_type":"hammer", "total":2, "finished":0} *)
+    induction t.
+    - admit. (* try hammer; admit.*)
+    - admit. (* try hammer; admit. *)
+    (*** MS END {"type": "proof", "proof_type":"hammer", "total":2, "finished":0} *)
+    Restart.
+  Proof.
+(*** MS BEGIN {"type": "proof", "proof_type":"mirrorsolve", "total":2} *)
+    induction t; 
+    prep_proof.
+    - reflect lookup_insert_shadow_emp; 
+      check_goal_unsat.
+    - reflect lookup_insert_shadow_node; 
+      check_goal_unsat.
+(*** MS END {"type": "proof", "proof_type":"mirrorsolve", "total":2} *)
+  Admitted.
+
+  (*** MS BEGIN {"type": "configuration", "config_type":"boilerplate"} *)
+  MetaCoq Quote Definition lookup_insert_same_emp := (
+    forall (k k' : Z) (d : V),
+    (forall (d0 : V) (x : Z) (l : tree V) (y : Z) (v : V) (r : tree V),
+     lookup d0 x (Node l y v r) = ite (x <? y)%Z (lookup d0 x l) (ite (x >? y)%Z (lookup d0 x r) v)) ->
+    (forall (d0 : V) (x : Z), lookup d0 x Emp = d0) ->
+    (forall (x : Z) (l : tree V) (y : Z) (v : V) (r : tree V),
+     bound x (Node l y v r) = ite (x <? y)%Z (bound x l) (ite (x >? y)%Z (bound x r) true)) ->
+    (forall x : Z, bound x Emp = false) ->
+    (forall (x : Z) (v : V) (l : tree V) (y : Z) (v' : V) (r : tree V),
+     insert x v (Node l y v' r) =
+     ite (x <? y)%Z (Node (insert x v l) y v' r) (ite (x >? y)%Z (Node l y v' (insert x v r)) (Node l x v r))) ->
+    (forall (x : Z) (v : V), insert x v Emp = Node Emp x v Emp) ->
+    (forall (l : tree V) (k0 : Z) (v : V) (r : tree V),
+     (lt_t k0 l /\ gt_t k0 r /\ ordered l /\ ordered r -> ordered (Node l k0 v r)) /\
+     (ordered (Node l k0 v r) -> lt_t k0 l /\ gt_t k0 r /\ ordered l /\ ordered r)) ->
+    ordered Emp ->
+    (forall (k0 : Z) (l : tree V) (k'0 : Z) (v : V) (r : tree V),
+     ((k'0 > k0)%Z /\ gt_t k0 l /\ gt_t k0 r -> gt_t k0 (Node l k'0 v r)) /\
+     (gt_t k0 (Node l k'0 v r) -> (k'0 > k0)%Z /\ gt_t k0 l /\ gt_t k0 r)) ->
+    (forall k0 : Z, gt_t k0 Emp) ->
+    (forall (k0 : Z) (l : tree V) (k'0 : Z) (v : V) (r : tree V),
+     ((k'0 < k0)%Z /\ lt_t k0 l /\ lt_t k0 r -> lt_t k0 (Node l k'0 v r)) /\
+     (lt_t k0 (Node l k'0 v r) -> (k'0 < k0)%Z /\ lt_t k0 l /\ lt_t k0 r)) ->
+    (forall k0 : Z, lt_t k0 Emp) -> lookup d k' (insert k (lookup d k Emp) Emp) = lookup d k' Emp    
+  ).
+  
+  MetaCoq Quote Definition lookup_insert_same_node := (
+    
+forall (k k' : Z) (d : V) (t1 : tree V) (k0 : Z) (v : V) (t2 : tree V),
+lookup d k' (insert k (lookup d k t1) t1) = lookup d k' t1 ->
+lookup d k' (insert k (lookup d k t2) t2) = lookup d k' t2 ->
+(forall (d0 : V) (x : Z) (l : tree V) (y : Z) (v0 : V) (r : tree V),
+ lookup d0 x (Node l y v0 r) = ite (x <? y)%Z (lookup d0 x l) (ite (x >? y)%Z (lookup d0 x r) v0)) ->
+(forall (d0 : V) (x : Z), lookup d0 x Emp = d0) ->
+(forall (x : Z) (l : tree V) (y : Z) (v0 : V) (r : tree V),
+ bound x (Node l y v0 r) = ite (x <? y)%Z (bound x l) (ite (x >? y)%Z (bound x r) true)) ->
+(forall x : Z, bound x Emp = false) ->
+(forall (x : Z) (v0 : V) (l : tree V) (y : Z) (v' : V) (r : tree V),
+ insert x v0 (Node l y v' r) =
+ ite (x <? y)%Z (Node (insert x v0 l) y v' r) (ite (x >? y)%Z (Node l y v' (insert x v0 r)) (Node l x v0 r))) ->
+(forall (x : Z) (v0 : V), insert x v0 Emp = Node Emp x v0 Emp) ->
+(forall (l : tree V) (k1 : Z) (v0 : V) (r : tree V),
+ (lt_t k1 l /\ gt_t k1 r /\ ordered l /\ ordered r -> ordered (Node l k1 v0 r)) /\
+ (ordered (Node l k1 v0 r) -> lt_t k1 l /\ gt_t k1 r /\ ordered l /\ ordered r)) ->
+ordered Emp ->
+(forall (k1 : Z) (l : tree V) (k'0 : Z) (v0 : V) (r : tree V),
+ ((k'0 > k1)%Z /\ gt_t k1 l /\ gt_t k1 r -> gt_t k1 (Node l k'0 v0 r)) /\
+ (gt_t k1 (Node l k'0 v0 r) -> (k'0 > k1)%Z /\ gt_t k1 l /\ gt_t k1 r)) ->
+(forall k1 : Z, gt_t k1 Emp) ->
+(forall (k1 : Z) (l : tree V) (k'0 : Z) (v0 : V) (r : tree V),
+ ((k'0 < k1)%Z /\ lt_t k1 l /\ lt_t k1 r -> lt_t k1 (Node l k'0 v0 r)) /\
+ (lt_t k1 (Node l k'0 v0 r) -> (k'0 < k1)%Z /\ lt_t k1 l /\ lt_t k1 r)) ->
+(forall k1 : Z, lt_t k1 Emp) ->
+lookup d k' (insert k (lookup d k (Node t1 k0 v t2)) (Node t1 k0 v t2)) = lookup d k' (Node t1 k0 v t2)
+  ).
+  (*** MS END {"type": "configuration", "config_type":"boilerplate"} *)
+
+  (** **** Exercise: 2 stars, standard, optional (lookup_insert_same) *)
+
+  (* hammer does not handle this one *)
+  (*** MS BEGIN {"type": "proof_definition"} *)
+  Lemma lookup_insert_same :
+    forall k k' d (t: tree V),
+      lookup d k' (insert k (lookup d k t) t) = lookup d k' t.
+  (*** MS END {"type": "proof_definition"} *)
+  Proof.
+    (*** MS BEGIN {"type": "proof", "proof_type":"manual"} *)
+    induction t; 
+    simpl in *;
+    intros.
+    - destruct (_ <? _)%Z eqn:?;
+      simpl in *;
+      trivial.
+      destruct (_ >? _)%Z eqn:?;
+      simpl in *;
+      trivial.
+    - destruct (_ <? _)%Z eqn:?;
+      simpl in *;
+      trivial.
+      + f_equal.
+        eauto.
+      + destruct (_ >? _)%Z eqn:?;
+        simpl in *;
+        trivial;
+        destruct (_ <? _)%Z eqn:?;
+        simpl.
+        * f_equal.
+          f_equal.
+          eauto.
+        * f_equal;
+          f_equal;
+          eauto.
+        * congruence.
+        * f_equal; [
+            Lia.lia
+            | f_equal
+          ].
+          Lia.lia.
+    (*** MS END {"type": "proof", "proof_type":"manual"} *)
+    Restart.
+  Proof.
+    (*** MS BEGIN {"type": "proof", "proof_type":"hammer", "total":2, "finished":0} *)
+    induction t.
+    - admit.
+    - admit.
+    (*** MS END {"type": "proof", "proof_type":"hammer", "total":2, "finished":0} *)
+    Restart.
+  Proof. 
+    (*** MS BEGIN {"type": "proof", "proof_type":"mirrorsolve", "total":2} *)
+    induction t; 
+    prep_proof.
+    - reflect lookup_insert_same_emp; 
+      check_goal_unsat.
+    - reflect lookup_insert_same_node; 
+      check_goal_unsat.
+    (*** MS END {"type": "proof", "proof_type":"mirrorsolve", "total":2} *)
+  Admitted.
+
+
+  (*** MS BEGIN {"type": "configuration", "config_type":"boilerplate"} *)
+  MetaCoq Quote Definition lookup_insert_permute_emp := (
+    forall (v1 v2 d : V) (k1 k2 k' : Z),
+(forall (d0 : V) (x : Z) (l : tree V) (y : Z) (v : V) (r : tree V),
+ lookup d0 x (Node l y v r) = ite (x <? y)%Z (lookup d0 x l) (ite (x >? y)%Z (lookup d0 x r) v)) ->
+(forall (d0 : V) (x : Z), lookup d0 x Emp = d0) ->
+(forall (x : Z) (l : tree V) (y : Z) (v : V) (r : tree V),
+ bound x (Node l y v r) = ite (x <? y)%Z (bound x l) (ite (x >? y)%Z (bound x r) true)) ->
+(forall x : Z, bound x Emp = false) ->
+(forall (x : Z) (v : V) (l : tree V) (y : Z) (v' : V) (r : tree V),
+ insert x v (Node l y v' r) =
+ ite (x <? y)%Z (Node (insert x v l) y v' r) (ite (x >? y)%Z (Node l y v' (insert x v r)) (Node l x v r))) ->
+(forall (x : Z) (v : V), insert x v Emp = Node Emp x v Emp) ->
+(forall (l : tree V) (k : Z) (v : V) (r : tree V),
+ (lt_t k l /\ gt_t k r /\ ordered l /\ ordered r -> ordered (Node l k v r)) /\
+ (ordered (Node l k v r) -> lt_t k l /\ gt_t k r /\ ordered l /\ ordered r)) ->
+ordered Emp ->
+(forall (k : Z) (l : tree V) (k'0 : Z) (v : V) (r : tree V),
+ ((k'0 > k)%Z /\ gt_t k l /\ gt_t k r -> gt_t k (Node l k'0 v r)) /\
+ (gt_t k (Node l k'0 v r) -> (k'0 > k)%Z /\ gt_t k l /\ gt_t k r)) ->
+(forall k : Z, gt_t k Emp) ->
+(forall (k : Z) (l : tree V) (k'0 : Z) (v : V) (r : tree V),
+ ((k'0 < k)%Z /\ lt_t k l /\ lt_t k r -> lt_t k (Node l k'0 v r)) /\
+ (lt_t k (Node l k'0 v r) -> (k'0 < k)%Z /\ lt_t k l /\ lt_t k r)) ->
+(forall k : Z, lt_t k Emp) ->
+k1 <> k2 -> lookup d k' (insert k1 v1 (insert k2 v2 Emp)) = lookup d k' (insert k2 v2 (insert k1 v1 Emp))
+).
+  
+  MetaCoq Quote Definition lookup_insert_permute_node := (
+    
+forall (v1 v2 d : V) (k1 k2 k' : Z) (t1 : tree V) (k : Z) (v : V) (t2 : tree V),
+(k1 <> k2 -> lookup d k' (insert k1 v1 (insert k2 v2 t1)) = lookup d k' (insert k2 v2 (insert k1 v1 t1))) ->
+(k1 <> k2 -> lookup d k' (insert k1 v1 (insert k2 v2 t2)) = lookup d k' (insert k2 v2 (insert k1 v1 t2))) ->
+(forall (d0 : V) (x : Z) (l : tree V) (y : Z) (v0 : V) (r : tree V),
+ lookup d0 x (Node l y v0 r) = ite (x <? y)%Z (lookup d0 x l) (ite (x >? y)%Z (lookup d0 x r) v0)) ->
+(forall (d0 : V) (x : Z), lookup d0 x Emp = d0) ->
+(forall (x : Z) (l : tree V) (y : Z) (v0 : V) (r : tree V),
+ bound x (Node l y v0 r) = ite (x <? y)%Z (bound x l) (ite (x >? y)%Z (bound x r) true)) ->
+(forall x : Z, bound x Emp = false) ->
+(forall (x : Z) (v0 : V) (l : tree V) (y : Z) (v' : V) (r : tree V),
+ insert x v0 (Node l y v' r) =
+ ite (x <? y)%Z (Node (insert x v0 l) y v' r) (ite (x >? y)%Z (Node l y v' (insert x v0 r)) (Node l x v0 r))) ->
+(forall (x : Z) (v0 : V), insert x v0 Emp = Node Emp x v0 Emp) ->
+(forall (l : tree V) (k0 : Z) (v0 : V) (r : tree V),
+ (lt_t k0 l /\ gt_t k0 r /\ ordered l /\ ordered r -> ordered (Node l k0 v0 r)) /\
+ (ordered (Node l k0 v0 r) -> lt_t k0 l /\ gt_t k0 r /\ ordered l /\ ordered r)) ->
+ordered Emp ->
+(forall (k0 : Z) (l : tree V) (k'0 : Z) (v0 : V) (r : tree V),
+ ((k'0 > k0)%Z /\ gt_t k0 l /\ gt_t k0 r -> gt_t k0 (Node l k'0 v0 r)) /\
+ (gt_t k0 (Node l k'0 v0 r) -> (k'0 > k0)%Z /\ gt_t k0 l /\ gt_t k0 r)) ->
+(forall k0 : Z, gt_t k0 Emp) ->
+(forall (k0 : Z) (l : tree V) (k'0 : Z) (v0 : V) (r : tree V),
+ ((k'0 < k0)%Z /\ lt_t k0 l /\ lt_t k0 r -> lt_t k0 (Node l k'0 v0 r)) /\
+ (lt_t k0 (Node l k'0 v0 r) -> (k'0 < k0)%Z /\ lt_t k0 l /\ lt_t k0 r)) ->
+(forall k0 : Z, lt_t k0 Emp) ->
+k1 <> k2 ->
+lookup d k' (insert k1 v1 (insert k2 v2 (Node t1 k v t2))) = lookup d k' (insert k2 v2 (insert k1 v1 (Node t1 k v t2)))
+  ).
+(*** MS END {"type": "configuration", "config_type":"boilerplate"} *)
+
+  (** **** Exercise: 2 stars, standard, optional (lookup_insert_permute) *)
+
+  (* hammer does not handle this one *)
+  (*** MS BEGIN {"type": "proof_definition"} *)
+  Lemma lookup_insert_permute :
+    forall v1 v2 d k1 k2 k' (t: tree V),
+      k1 <> k2 ->
+      lookup d k' (insert k1 v1 (insert k2 v2 t))
+      = lookup d k' (insert k2 v2 (insert k1 v1 t)).
+  (*** MS END {"type": "proof_definition"} *)
+  Proof. 
+    (*** MS BEGIN {"type": "proof", "proof_type":"manual"} *)
+    induction t;
+    simpl in *;
+    intros.
+    - destruct (_ <? _)%Z eqn:?;  
+      simpl.
+      * assert ((k2 <? k1)%Z = false) by Lia.lia.
+        assert ((k2 >? k1)%Z = true) by Lia.lia.
+        erewrite H0.
+        erewrite H1.
+        simpl.
+        destruct (k' <? k2)%Z eqn:?;
+        simpl; [
+          trivial
+          | 
+        ].
+        destruct (k' <? k1)%Z eqn:?;
+        assert ((k' >? k1)%Z = true) by Lia.lia;
+        erewrite H2;
+        simpl.
+        + destruct (k' >? k2)%Z eqn:?;
+          simpl; [
+              trivial
+            | Lia.lia
+          ].
+        + destruct (k' >? k2)%Z eqn:?;
+          simpl;
+          trivial.
+      * assert ((k2 <? k1)%Z = true) by Lia.lia.
+        assert ((k2 >? k1)%Z = false) by Lia.lia.
+        erewrite H0.
+        erewrite H1.
+        simpl.
+        destruct (k' <? k1)%Z eqn:?;
+        simpl; 
+        assert ((k1 >? k2)%Z = true) by Lia.lia;
+        erewrite H2;
+        simpl.
+        + f_equal.
+          f_equal.
+          erewrite Heqb0;
+          trivial.
+        + destruct (k' <? k2)%Z eqn:?;
+          try Lia.lia;
+          assert ((k' >? k2)%Z = true) by Lia.lia;
+          erewrite H3;
+          erewrite Heqb0;
+          simpl;
+          f_equal.
+    - destruct (k2 <? k)%Z eqn:?;
+      destruct (k2 >? k)%Z eqn:?;
+      destruct (k1 <? k)%Z eqn:?;
+      destruct (k1 >? k)%Z eqn:?;
+      simpl;
+      try Lia.lia.
+      * erewrite Heqb1.
+        erewrite Heqb.
+        simpl.
+        f_equal;  
+        eauto.
+      * erewrite Heqb1.
+        erewrite Heqb0.
+        erewrite Heqb2.
+        erewrite Heqb.
+        simpl.
+        f_equal.
+      * erewrite Heqb1.
+        erewrite Heqb2.
+        simpl.
+        destruct (k2 <? k1)%Z eqn:?;
+        simpl;
+        trivial.
+        assert ((k2 >? k1)%Z = true) by Lia.lia.
+        erewrite H0.
+        simpl.
+        f_equal.
+        + eapply lookup_insert_neq;
+          Lia.lia.
+        + f_equal.
+          erewrite lookup_insert_neq;
+          trivial.
+          Lia.lia.
+      * erewrite Heqb1;
+        erewrite Heqb;
+        erewrite Heqb0;
+        erewrite Heqb2;
+        simpl.
+        f_equal.
+      * erewrite Heqb1;
+        erewrite Heqb;
+        erewrite Heqb0;
+        erewrite Heqb2;
+        simpl.
+        f_equal.
+        f_equal.
+        eapply IHt2.
+        trivial.
+      * erewrite Heqb1;
+        erewrite Heqb2;
+        simpl;
+        destruct (k2 <? k1)%Z eqn:?;
+        simpl;
+        try Lia.lia.
+        assert ((k2 >? k1)%Z = true) by Lia.lia.
+        erewrite H0.
+        simpl.
+        f_equal.
+      * erewrite Heqb;
+        erewrite Heqb0;
+        simpl.
+        destruct (k1 <? k2)%Z eqn:?;
+        simpl; [
+            f_equal
+          |
+        ].
+        assert ((k1 >? k2)%Z = true) by Lia.lia.
+        erewrite H0.
+        simpl.
+        f_equal;
+        try Lia.lia.
+      * erewrite Heqb;
+        erewrite Heqb0;
+        simpl.
+        destruct (k1 <? k2)%Z eqn:?;
+        simpl; [
+            Lia.lia
+          |
+        ].
+        assert ((k1 >? k2)%Z = true) by Lia.lia.
+        erewrite H0.
+        simpl.
+        f_equal.
+    (*** MS END {"type": "proof", "proof_type":"manual"} *)
+    Restart.
+  Proof.
+    (*** MS BEGIN {"type": "proof", "proof_type":"hammer", "total":2, "finished":0} *)
+    induction t.
+    - admit. (* hammer. *)
+    - admit. (* hammer. *)
+    (*** MS END {"type": "proof", "proof_type":"hammer", "total":2, "finished":0} *)
+  Restart.
+  (*** MS BEGIN {"type": "proof", "proof_type":"mirrorsolve", "total":2} *)
+    induction t; 
+    prep_proof.
+    - reflect lookup_insert_permute_emp; 
+      check_goal_unsat.
+    - reflect lookup_insert_permute_node; 
+      check_goal_unsat.
+  (*** MS END {"type": "proof", "proof_type":"mirrorsolve", "total":2} *)
+  Admitted.
+
+(** Our ability to prove these lemmas without reference to the
+    underlying tree implementation demonstrates they hold for any map
+    implementation that satisfies the three basic equations. *)
+
+(** Each of these lemmas just proved was phrased as an equality
+    between the results of looking up an arbitrary key [k'] in two
+    maps.  But the lemmas for the function-based maps were phrased as
+    direct equalities between the maps themselves.
+
+    Could we state the tree lemmas with direct equalities?  For
+    [insert_shadow], the answer is yes: *)
+
+(*** MS BEGIN {"type": "configuration", "config_type":"boilerplate"} *)
+    MetaCoq Quote Definition insert_shadow_equality_emp := (
+      (forall (d : V) (x : Z) (l : tree V) (y : Z) (v : V) (r : tree V),
+ lookup d x (Node l y v r) = ite (x <? y)%Z (lookup d x l) (ite (x >? y)%Z (lookup d x r) v)) ->
+(forall (d : V) (x : Z), lookup d x Emp = d) ->
+(forall (x : Z) (l : tree V) (y : Z) (v : V) (r : tree V),
+ bound x (Node l y v r) = ite (x <? y)%Z (bound x l) (ite (x >? y)%Z (bound x r) true)) ->
+(forall x : Z, bound x Emp = false) ->
+(forall (x : Z) (v : V) (l : tree V) (y : Z) (v' : V) (r : tree V),
+ insert x v (Node l y v' r) =
+ ite (x <? y)%Z (Node (insert x v l) y v' r) (ite (x >? y)%Z (Node l y v' (insert x v r)) (Node l x v r))) ->
+(forall (x : Z) (v : V), insert x v Emp = Node Emp x v Emp) ->
+(forall (l : tree V) (k : Z) (v : V) (r : tree V),
+ (lt_t k l /\ gt_t k r /\ ordered l /\ ordered r -> ordered (Node l k v r)) /\
+ (ordered (Node l k v r) -> lt_t k l /\ gt_t k r /\ ordered l /\ ordered r)) ->
+ordered Emp ->
+(forall (k : Z) (l : tree V) (k' : Z) (v : V) (r : tree V),
+ ((k' > k)%Z /\ gt_t k l /\ gt_t k r -> gt_t k (Node l k' v r)) /\
+ (gt_t k (Node l k' v r) -> (k' > k)%Z /\ gt_t k l /\ gt_t k r)) ->
+(forall k : Z, gt_t k Emp) ->
+(forall (k : Z) (l : tree V) (k' : Z) (v : V) (r : tree V),
+ ((k' < k)%Z /\ lt_t k l /\ lt_t k r -> lt_t k (Node l k' v r)) /\
+ (lt_t k (Node l k' v r) -> (k' < k)%Z /\ lt_t k l /\ lt_t k r)) ->
+(forall k : Z, lt_t k Emp) -> forall (k : Z) (v v' : V), insert k v (insert k v' Emp) = insert k v Emp
+  ).
+    
+    MetaCoq Quote Definition insert_shadow_equality_node := (
+      
+forall (t1 : tree V) (k : Z) (v : V) (t2 : tree V),
+(forall (k0 : Z) (v0 v' : V), insert k0 v0 (insert k0 v' t1) = insert k0 v0 t1) ->
+(forall (k0 : Z) (v0 v' : V), insert k0 v0 (insert k0 v' t2) = insert k0 v0 t2) ->
+(forall (d : V) (x : Z) (l : tree V) (y : Z) (v0 : V) (r : tree V),
+ lookup d x (Node l y v0 r) = ite (x <? y)%Z (lookup d x l) (ite (x >? y)%Z (lookup d x r) v0)) ->
+(forall (d : V) (x : Z), lookup d x Emp = d) ->
+(forall (x : Z) (l : tree V) (y : Z) (v0 : V) (r : tree V),
+ bound x (Node l y v0 r) = ite (x <? y)%Z (bound x l) (ite (x >? y)%Z (bound x r) true)) ->
+(forall x : Z, bound x Emp = false) ->
+(forall (x : Z) (v0 : V) (l : tree V) (y : Z) (v' : V) (r : tree V),
+ insert x v0 (Node l y v' r) =
+ ite (x <? y)%Z (Node (insert x v0 l) y v' r) (ite (x >? y)%Z (Node l y v' (insert x v0 r)) (Node l x v0 r))) ->
+(forall (x : Z) (v0 : V), insert x v0 Emp = Node Emp x v0 Emp) ->
+(forall (l : tree V) (k0 : Z) (v0 : V) (r : tree V),
+ (lt_t k0 l /\ gt_t k0 r /\ ordered l /\ ordered r -> ordered (Node l k0 v0 r)) /\
+ (ordered (Node l k0 v0 r) -> lt_t k0 l /\ gt_t k0 r /\ ordered l /\ ordered r)) ->
+ordered Emp ->
+(forall (k0 : Z) (l : tree V) (k' : Z) (v0 : V) (r : tree V),
+ ((k' > k0)%Z /\ gt_t k0 l /\ gt_t k0 r -> gt_t k0 (Node l k' v0 r)) /\
+ (gt_t k0 (Node l k' v0 r) -> (k' > k0)%Z /\ gt_t k0 l /\ gt_t k0 r)) ->
+(forall k0 : Z, gt_t k0 Emp) ->
+(forall (k0 : Z) (l : tree V) (k' : Z) (v0 : V) (r : tree V),
+ ((k' < k0)%Z /\ lt_t k0 l /\ lt_t k0 r -> lt_t k0 (Node l k' v0 r)) /\
+ (lt_t k0 (Node l k' v0 r) -> (k' < k0)%Z /\ lt_t k0 l /\ lt_t k0 r)) ->
+(forall k0 : Z, lt_t k0 Emp) ->
+forall (k0 : Z) (v0 v' : V), insert k0 v0 (insert k0 v' (Node t1 k v t2)) = insert k0 v0 (Node t1 k v t2)
+    ).
+(*** MS END {"type": "configuration", "config_type":"boilerplate"} *)
+
+
+  (* hammer does not handle this one *)
+  (*** MS BEGIN {"type": "proof_definition"} *)
+  Lemma insert_shadow_equality : 
+    forall (t: tree V) k v v',
+      insert k v (insert k v' t) = insert k v t.
+  (*** MS END {"type": "proof_definition"} *)
+  Proof.
+    (*** MS BEGIN {"type": "proof", "proof_type":"manual"} *)
+    induction t;
+    simpl in *;
+    intros.
+    - assert ((k <? k)%Z = false) by Lia.lia;
+      assert ((k >? k)%Z = false) by Lia.lia;
+      erewrite H;
+      erewrite H0;
+      simpl.
+      trivial.
+    - destruct (_ <? _)%Z eqn:?;
+      simpl.
+      * erewrite Heqb.
+        simpl.
+        f_equal.
+        eapply IHt1.
+      * destruct (k0 >? k)%Z eqn:?;
+        simpl.
+        + erewrite Heqb.
+          erewrite Heqb0.
+          simpl.
+          f_equal.
+          eapply IHt2.
+        + assert ((k0 <? k0)%Z = false) by Lia.lia.
+          erewrite H;
+          simpl.
+          assert ((k0 >? k0)%Z = false) by Lia.lia;
+          erewrite H0;
+          simpl.
+          trivial.
+    (*** MS END {"type": "proof", "proof_type":"manual"} *)
+    Restart.
+  Proof.
+    (*** MS BEGIN {"type": "proof", "proof_type":"hammer", "total":2, "finished":0} *)
+    induction t.
+    - admit. (* hammer. *)
+    - admit. (* hammer. *)
+    (*** MS END {"type": "proof", "proof_type":"hammer", "total":2, "finished":0} *)
+    Restart.
+  Proof.
+    (*** MS BEGIN {"type": "proof", "proof_type":"mirrorsolve", "total":2} *)
+    induction t; 
+    prep_proof.
+    - reflect insert_shadow_equality_emp; 
+      check_goal_unsat.
+    - reflect insert_shadow_equality_node; 
+      check_goal_unsat.
+    (*** MS END {"type": "proof", "proof_type":"mirrorsolve", "total":2} *)
+  Admitted.
+
+(** But the other two direct equalities on BSTs do not necessarily
+    hold. *)
+
+(** **** Exercise: 3 stars, standard, optional (direct_equalities_break) *)
+
+(** Prove that the other equalities do not hold.  Hint: find a counterexample
+    first on paper, then use the [exists] tactic to instantiate the theorem
+    on your counterexample.  The simpler your counterexample, the simpler
+    the rest of the proof will be. *)
+
+(* Lemma insert_same_equality_breaks :
+  exists (V : Type) (d : V) (t : tree V) (k : key),
+      insert k (lookup d k t) t <> t.
+Proof.
+  (* FILL IN HERE *) Admitted.
+
+Lemma insert_permute_equality_breaks :
+  exists (V : Type) (v1 v2 : V) (k1 k2 : key) (t : tree V),
+    k1 <> k2 /\ insert k1 v1 (insert k2 v2 t) <> insert k2 v2 (insert k1 v1 t).
+Proof.
+  (* FILL IN HERE *) Admitted. *)
+
+(** [] *)
+
+(** some custom stuff, about balance and that insert preserves the balance of the tree **)
+
+(*** MS BEGIN {"type": "configuration", "config_type":"boilerplate"} *)
+MetaCoq Quote Definition insert_left_lt_emp := (
+  
+(forall (d : V) (x : Z) (l : tree V) (y : Z) (v : V) (r : tree V),
+lookup d x (Node l y v r) = ite (x <? y)%Z (lookup d x l) (ite (x >? y)%Z (lookup d x r) v)) ->
+(forall (d : V) (x : Z), lookup d x Emp = d) ->
+(forall (x : Z) (l : tree V) (y : Z) (v : V) (r : tree V),
+bound x (Node l y v r) = ite (x <? y)%Z (bound x l) (ite (x >? y)%Z (bound x r) true)) ->
+(forall x : Z, bound x Emp = false) ->
+(forall (x : Z) (v : V) (l : tree V) (y : Z) (v' : V) (r : tree V),
+insert x v (Node l y v' r) =
+ite (x <? y)%Z (Node (insert x v l) y v' r) (ite (x >? y)%Z (Node l y v' (insert x v r)) (Node l x v r))) ->
+(forall (x : Z) (v : V), insert x v Emp = Node Emp x v Emp) ->
+(forall (l : tree V) (k : Z) (v : V) (r : tree V),
+(lt_t k l /\ gt_t k r /\ ordered l /\ ordered r -> ordered (Node l k v r)) /\
+(ordered (Node l k v r) -> lt_t k l /\ gt_t k r /\ ordered l /\ ordered r)) ->
+ordered Emp ->
+(forall (k : Z) (l : tree V) (k' : Z) (v : V) (r : tree V),
+((k' > k)%Z /\ gt_t k l /\ gt_t k r -> gt_t k (Node l k' v r)) /\
+(gt_t k (Node l k' v r) -> (k' > k)%Z /\ gt_t k l /\ gt_t k r)) ->
+(forall k : Z, gt_t k Emp) ->
+(forall (k : Z) (l : tree V) (k' : Z) (v : V) (r : tree V),
+((k' < k)%Z /\ lt_t k l /\ lt_t k r -> lt_t k (Node l k' v r)) /\
+(lt_t k (Node l k' v r) -> (k' < k)%Z /\ lt_t k l /\ lt_t k r)) ->
+(forall k : Z, lt_t k Emp) -> forall (k k' : Z) (v : V), (k < k')%Z -> lt_t k' Emp -> lt_t k' (insert k v Emp)
+).
+
+MetaCoq Quote Definition insert_left_lt_node := (
+  forall (l1 : tree V) (k : Z) (v : V) (l2 : tree V),
+(forall (k0 k' : Z) (v0 : V), (k0 < k')%Z -> lt_t k' l1 -> lt_t k' (insert k0 v0 l1)) ->
+(forall (k0 k' : Z) (v0 : V), (k0 < k')%Z -> lt_t k' l2 -> lt_t k' (insert k0 v0 l2)) ->
+(forall (d : V) (x : Z) (l : tree V) (y : Z) (v0 : V) (r : tree V),
+ lookup d x (Node l y v0 r) = ite (x <? y)%Z (lookup d x l) (ite (x >? y)%Z (lookup d x r) v0)) ->
+(forall (d : V) (x : Z), lookup d x Emp = d) ->
+(forall (x : Z) (l : tree V) (y : Z) (v0 : V) (r : tree V),
+ bound x (Node l y v0 r) = ite (x <? y)%Z (bound x l) (ite (x >? y)%Z (bound x r) true)) ->
+(forall x : Z, bound x Emp = false) ->
+(forall (x : Z) (v0 : V) (l : tree V) (y : Z) (v' : V) (r : tree V),
+ insert x v0 (Node l y v' r) =
+ ite (x <? y)%Z (Node (insert x v0 l) y v' r) (ite (x >? y)%Z (Node l y v' (insert x v0 r)) (Node l x v0 r))) ->
+(forall (x : Z) (v0 : V), insert x v0 Emp = Node Emp x v0 Emp) ->
+(forall (l : tree V) (k0 : Z) (v0 : V) (r : tree V),
+ (lt_t k0 l /\ gt_t k0 r /\ ordered l /\ ordered r -> ordered (Node l k0 v0 r)) /\
+ (ordered (Node l k0 v0 r) -> lt_t k0 l /\ gt_t k0 r /\ ordered l /\ ordered r)) ->
+ordered Emp ->
+(forall (k0 : Z) (l : tree V) (k' : Z) (v0 : V) (r : tree V),
+ ((k' > k0)%Z /\ gt_t k0 l /\ gt_t k0 r -> gt_t k0 (Node l k' v0 r)) /\
+ (gt_t k0 (Node l k' v0 r) -> (k' > k0)%Z /\ gt_t k0 l /\ gt_t k0 r)) ->
+(forall k0 : Z, gt_t k0 Emp) ->
+(forall (k0 : Z) (l : tree V) (k' : Z) (v0 : V) (r : tree V),
+ ((k' < k0)%Z /\ lt_t k0 l /\ lt_t k0 r -> lt_t k0 (Node l k' v0 r)) /\
+ (lt_t k0 (Node l k' v0 r) -> (k' < k0)%Z /\ lt_t k0 l /\ lt_t k0 r)) ->
+(forall k0 : Z, lt_t k0 Emp) ->
+forall (k0 k' : Z) (v0 : V), (k0 < k')%Z -> lt_t k' (Node l1 k v l2) -> lt_t k' (insert k0 v0 (Node l1 k v l2))
+).
+(*** MS END {"type": "configuration", "config_type":"boilerplate"} *)
+
+(* unfortunately we can't handle the recursive case *)
+SetSMTSolver "cvc5".
+(*** MS BEGIN {"type": "proof_definition"} *)
+Lemma insert_left_lt : 
+  forall (l: tree V) k k' v, 
+    (k < k')%Z -> 
+    lt_t k' l -> 
+    lt_t k' (insert k v l).
+(*** MS END {"type": "proof_definition"} *)
+Proof. 
+  (*** MS BEGIN {"type": "proof", "proof_type":"manual"} *)
+  induction l;
+  intros; 
+  simpl in *.
+  - intuition.
+  - destruct (k0 <? k)%Z eqn:?;
+    simpl in *; [
+        intuition 
+      | 
+    ].
+    destruct (k0 >? k)%Z eqn:?;
+    simpl in *; 
+    intuition.
+  (*** MS END {"type": "proof", "proof_type":"manual"} *)
+  Restart.
+Proof.
+  (*** MS BEGIN {"type": "proof", "proof_type":"hammer", "total":2, "finished":1} *)
+  induction l.
+  - hammer.
+  - admit. (* hammer. *)
+  (*** MS END {"type": "proof", "proof_type":"hammer", "total":2, "finished":1} *)
+  Restart.
+Proof.
+  (*** MS BEGIN {"type": "proof", "proof_type":"mirrorsolve", "total":2} *)
+  induction l;
+  prep_proof.
+  - reflect insert_left_lt_emp; 
+    check_goal_unsat.
+  - reflect insert_left_lt_node;
+    check_goal_unsat.
+(*** MS END {"type": "proof", "proof_type":"mirrorsolve", "total":2} *)
+Admitted.
+
+(*** MS BEGIN {"type": "configuration", "config_type":"boilerplate"} *)
+MetaCoq Quote Definition insert_right_lt_emp := (
+  
+(forall (d : V) (x : Z) (l : tree V) (y : Z) (v : V) (r : tree V),
+lookup d x (Node l y v r) = ite (x <? y)%Z (lookup d x l) (ite (x >? y)%Z (lookup d x r) v)) ->
+(forall (d : V) (x : Z), lookup d x Emp = d) ->
+(forall (x : Z) (l : tree V) (y : Z) (v : V) (r : tree V),
+bound x (Node l y v r) = ite (x <? y)%Z (bound x l) (ite (x >? y)%Z (bound x r) true)) ->
+(forall x : Z, bound x Emp = false) ->
+(forall (x : Z) (v : V) (l : tree V) (y : Z) (v' : V) (r : tree V),
+insert x v (Node l y v' r) =
+ite (x <? y)%Z (Node (insert x v l) y v' r) (ite (x >? y)%Z (Node l y v' (insert x v r)) (Node l x v r))) ->
+(forall (x : Z) (v : V), insert x v Emp = Node Emp x v Emp) ->
+(forall (l : tree V) (k : Z) (v : V) (r : tree V),
+(lt_t k l /\ gt_t k r /\ ordered l /\ ordered r -> ordered (Node l k v r)) /\
+(ordered (Node l k v r) -> lt_t k l /\ gt_t k r /\ ordered l /\ ordered r)) ->
+ordered Emp ->
+(forall (k : Z) (l : tree V) (k' : Z) (v : V) (r : tree V),
+((k' > k)%Z /\ gt_t k l /\ gt_t k r -> gt_t k (Node l k' v r)) /\
+(gt_t k (Node l k' v r) -> (k' > k)%Z /\ gt_t k l /\ gt_t k r)) ->
+(forall k : Z, gt_t k Emp) ->
+(forall (k : Z) (l : tree V) (k' : Z) (v : V) (r : tree V),
+((k' < k)%Z /\ lt_t k l /\ lt_t k r -> lt_t k (Node l k' v r)) /\
+(lt_t k (Node l k' v r) -> (k' < k)%Z /\ lt_t k l /\ lt_t k r)) ->
+(forall k : Z, lt_t k Emp) -> forall (k k' : Z) (v : V), (k' < k)%Z -> gt_t k' Emp -> gt_t k' (insert k v Emp)
+).
+
+MetaCoq Quote Definition insert_right_lt_node := (
+  
+forall (r1 : tree V) (k : Z) (v : V) (r2 : tree V),
+(forall (k0 k' : Z) (v0 : V), (k' < k0)%Z -> gt_t k' r1 -> gt_t k' (insert k0 v0 r1)) ->
+(forall (k0 k' : Z) (v0 : V), (k' < k0)%Z -> gt_t k' r2 -> gt_t k' (insert k0 v0 r2)) ->
+(forall (d : V) (x : Z) (l : tree V) (y : Z) (v0 : V) (r : tree V),
+ lookup d x (Node l y v0 r) = ite (x <? y)%Z (lookup d x l) (ite (x >? y)%Z (lookup d x r) v0)) ->
+(forall (d : V) (x : Z), lookup d x Emp = d) ->
+(forall (x : Z) (l : tree V) (y : Z) (v0 : V) (r : tree V),
+ bound x (Node l y v0 r) = ite (x <? y)%Z (bound x l) (ite (x >? y)%Z (bound x r) true)) ->
+(forall x : Z, bound x Emp = false) ->
+(forall (x : Z) (v0 : V) (l : tree V) (y : Z) (v' : V) (r : tree V),
+ insert x v0 (Node l y v' r) =
+ ite (x <? y)%Z (Node (insert x v0 l) y v' r) (ite (x >? y)%Z (Node l y v' (insert x v0 r)) (Node l x v0 r))) ->
+(forall (x : Z) (v0 : V), insert x v0 Emp = Node Emp x v0 Emp) ->
+(forall (l : tree V) (k0 : Z) (v0 : V) (r : tree V),
+ (lt_t k0 l /\ gt_t k0 r /\ ordered l /\ ordered r -> ordered (Node l k0 v0 r)) /\
+ (ordered (Node l k0 v0 r) -> lt_t k0 l /\ gt_t k0 r /\ ordered l /\ ordered r)) ->
+ordered Emp ->
+(forall (k0 : Z) (l : tree V) (k' : Z) (v0 : V) (r : tree V),
+ ((k' > k0)%Z /\ gt_t k0 l /\ gt_t k0 r -> gt_t k0 (Node l k' v0 r)) /\
+ (gt_t k0 (Node l k' v0 r) -> (k' > k0)%Z /\ gt_t k0 l /\ gt_t k0 r)) ->
+(forall k0 : Z, gt_t k0 Emp) ->
+(forall (k0 : Z) (l : tree V) (k' : Z) (v0 : V) (r : tree V),
+ ((k' < k0)%Z /\ lt_t k0 l /\ lt_t k0 r -> lt_t k0 (Node l k' v0 r)) /\
+ (lt_t k0 (Node l k' v0 r) -> (k' < k0)%Z /\ lt_t k0 l /\ lt_t k0 r)) ->
+(forall k0 : Z, lt_t k0 Emp) ->
+forall (k0 k' : Z) (v0 : V), (k' < k0)%Z -> gt_t k' (Node r1 k v r2) -> gt_t k' (insert k0 v0 (Node r1 k v r2))
+).
+(*** MS END {"type": "configuration", "config_type":"boilerplate"} *)
+
+(*** MS BEGIN {"type": "proof_definition"} *)
+Lemma insert_right_lt : 
+  forall (r: tree V) k k' v, 
+    (k' < k)%Z -> 
+    gt_t k' r -> 
+    gt_t k' (insert k v r).
+(*** MS END {"type": "proof_definition"} *)
+Proof.
+  (*** MS BEGIN {"type": "proof", "proof_type":"manual"} *)
+  induction r;
+  intros; 
+  simpl in *.
+  - intuition.
+  - destruct (k0 <? k)%Z eqn:?;
+    simpl in *; [
+        intuition 
+      | 
+    ].
+    destruct (k0 >? k)%Z eqn:?;
+    simpl in *; 
+    intuition.
+  (*** MS END {"type": "proof", "proof_type":"manual"} *)
+  Restart.
+Proof.
+  (*** MS BEGIN {"type": "proof", "proof_type":"hammer", "total":2, "finished":0} *)
+  induction r.
+  - admit. (* hammer. *)
+  - admit. (* hammer. *)
+  (*** MS END {"type": "proof", "proof_type":"hammer", "total":2, "finished":0} *)
+  Restart.
+Proof.
+  (*** MS BEGIN {"type": "proof", "proof_type":"mirrorsolve", "total":2} *)
+  induction r;
+  prep_proof.
+  - reflect insert_right_lt_emp; 
+    check_goal_unsat.
+  - reflect insert_right_lt_node; 
+    check_goal_unsat.
+  (*** MS END {"type": "proof", "proof_type":"mirrorsolve", "total":2} *)
+Admitted.
+(*** MS BEGIN {"type": "configuration", "config_type":"tactics"} *)
+Ltac prep_proof' := Utils.pose_all (tt, insert_left_lt, insert_right_lt); 
+  prep_proof.
+(*** MS END {"type": "configuration", "config_type":"tactics"} *)
+
+(*** MS BEGIN {"type": "configuration", "config_type":"boilerplate"} *)
+MetaCoq Quote Definition insert_ordered_left_emp := (
+  
+(forall (r : tree V) (k k' : Z) (v : V), (k' < k)%Z -> gt_t k' r -> gt_t k' (insert k v r)) ->
+(forall (l : tree V) (k k' : Z) (v : V), (k < k')%Z -> lt_t k' l -> lt_t k' (insert k v l)) ->
+(forall (d : V) (x : Z) (l : tree V) (y : Z) (v : V) (r : tree V),
+ lookup d x (Node l y v r) = ite (x <? y)%Z (lookup d x l) (ite (x >? y)%Z (lookup d x r) v)) ->
+(forall (d : V) (x : Z), lookup d x Emp = d) ->
+(forall (x : Z) (l : tree V) (y : Z) (v : V) (r : tree V),
+ bound x (Node l y v r) = ite (x <? y)%Z (bound x l) (ite (x >? y)%Z (bound x r) true)) ->
+(forall x : Z, bound x Emp = false) ->
+(forall (x : Z) (v : V) (l : tree V) (y : Z) (v' : V) (r : tree V),
+ insert x v (Node l y v' r) =
+ ite (x <? y)%Z (Node (insert x v l) y v' r) (ite (x >? y)%Z (Node l y v' (insert x v r)) (Node l x v r))) ->
+(forall (x : Z) (v : V), insert x v Emp = Node Emp x v Emp) ->
+(forall (l : tree V) (k : Z) (v : V) (r : tree V),
+ (lt_t k l /\ gt_t k r /\ ordered l /\ ordered r -> ordered (Node l k v r)) /\
+ (ordered (Node l k v r) -> lt_t k l /\ gt_t k r /\ ordered l /\ ordered r)) ->
+ordered Emp ->
+(forall (k : Z) (l : tree V) (k' : Z) (v : V) (r : tree V),
+ ((k' > k)%Z /\ gt_t k l /\ gt_t k r -> gt_t k (Node l k' v r)) /\
+ (gt_t k (Node l k' v r) -> (k' > k)%Z /\ gt_t k l /\ gt_t k r)) ->
+(forall k : Z, gt_t k Emp) ->
+(forall (k : Z) (l : tree V) (k' : Z) (v : V) (r : tree V),
+ ((k' < k)%Z /\ lt_t k l /\ lt_t k r -> lt_t k (Node l k' v r)) /\
+ (lt_t k (Node l k' v r) -> (k' < k)%Z /\ lt_t k l /\ lt_t k r)) ->
+(forall k : Z, lt_t k Emp) ->
+forall (k k' : Z) (v : V), (k < k')%Z -> lt_t k' Emp -> ordered Emp -> ordered (insert k v Emp)
+).
+
+MetaCoq Quote Definition insert_ordered_left_node := (
+  forall (l1 : tree V) (k : Z) (v : V) (l2 : tree V),
+(forall (k0 k' : Z) (v0 : V), (k0 < k')%Z -> lt_t k' l1 -> ordered l1 -> ordered (insert k0 v0 l1)) ->
+(forall (k0 k' : Z) (v0 : V), (k0 < k')%Z -> lt_t k' l2 -> ordered l2 -> ordered (insert k0 v0 l2)) ->
+(forall (r : tree V) (k0 k' : Z) (v0 : V), (k' < k0)%Z -> gt_t k' r -> gt_t k' (insert k0 v0 r)) ->
+(forall (l : tree V) (k0 k' : Z) (v0 : V), (k0 < k')%Z -> lt_t k' l -> lt_t k' (insert k0 v0 l)) ->
+(forall (d : V) (x : Z) (l : tree V) (y : Z) (v0 : V) (r : tree V),
+ lookup d x (Node l y v0 r) = ite (x <? y)%Z (lookup d x l) (ite (x >? y)%Z (lookup d x r) v0)) ->
+(forall (d : V) (x : Z), lookup d x Emp = d) ->
+(forall (x : Z) (l : tree V) (y : Z) (v0 : V) (r : tree V),
+ bound x (Node l y v0 r) = ite (x <? y)%Z (bound x l) (ite (x >? y)%Z (bound x r) true)) ->
+(forall x : Z, bound x Emp = false) ->
+(forall (x : Z) (v0 : V) (l : tree V) (y : Z) (v' : V) (r : tree V),
+ insert x v0 (Node l y v' r) =
+ ite (x <? y)%Z (Node (insert x v0 l) y v' r) (ite (x >? y)%Z (Node l y v' (insert x v0 r)) (Node l x v0 r))) ->
+(forall (x : Z) (v0 : V), insert x v0 Emp = Node Emp x v0 Emp) ->
+(forall (l : tree V) (k0 : Z) (v0 : V) (r : tree V),
+ (lt_t k0 l /\ gt_t k0 r /\ ordered l /\ ordered r -> ordered (Node l k0 v0 r)) /\
+ (ordered (Node l k0 v0 r) -> lt_t k0 l /\ gt_t k0 r /\ ordered l /\ ordered r)) ->
+ordered Emp ->
+(forall (k0 : Z) (l : tree V) (k' : Z) (v0 : V) (r : tree V),
+ ((k' > k0)%Z /\ gt_t k0 l /\ gt_t k0 r -> gt_t k0 (Node l k' v0 r)) /\
+ (gt_t k0 (Node l k' v0 r) -> (k' > k0)%Z /\ gt_t k0 l /\ gt_t k0 r)) ->
+(forall k0 : Z, gt_t k0 Emp) ->
+(forall (k0 : Z) (l : tree V) (k' : Z) (v0 : V) (r : tree V),
+ ((k' < k0)%Z /\ lt_t k0 l /\ lt_t k0 r -> lt_t k0 (Node l k' v0 r)) /\
+ (lt_t k0 (Node l k' v0 r) -> (k' < k0)%Z /\ lt_t k0 l /\ lt_t k0 r)) ->
+(forall k0 : Z, lt_t k0 Emp) ->
+forall (k0 k' : Z) (v0 : V),
+(k0 < k')%Z -> lt_t k' (Node l1 k v l2) -> ordered (Node l1 k v l2) -> ordered (insert k0 v0 (Node l1 k v l2))
+).
+
+(*** MS END {"type": "configuration", "config_type":"boilerplate"} *)
+
+(*** MS BEGIN {"type": "proof_definition"} *)
+Lemma insert_ordered_left :
+  forall (l: tree V) k k' v, 
+    (k < k')%Z -> 
+    lt_t k' l -> 
+    ordered l ->
+    ordered (insert k v l).
+(*** MS END {"type": "proof_definition"} *)
+Proof.
+  (*** MS BEGIN {"type": "proof", "proof_type":"manual"} *)
+  induction l;
+  intros;
+  simpl in *.
+  - intuition.
+  - destruct (k0 <? k)%Z eqn:?;
+    simpl in *.
+    * intuition.
+      eapply insert_left_lt;
+      eauto.
+      Lia.lia.
+    * destruct (k0 >? k)%Z eqn:?;
+      simpl in *; 
+      intuition.
+      + eapply insert_right_lt;
+        intuition.
+      + assert (k0 = k) by Lia.lia.
+        subst.
+        trivial.
+      + assert (k0 = k) by Lia.lia.
+        subst.
+        trivial.
+  (*** MS END {"type": "proof", "proof_type":"manual"} *)
+  Restart.
+Proof.
+  (*** MS BEGIN {"type": "proof", "proof_type":"hammer", "total":2, "finished":1} *)
+  induction l.
+  - hammer.
+  - admit. (* hammer. *)
+  (*** MS END {"type": "proof", "proof_type":"hammer", "total":2, "finished":1} *)
+  Restart.
+Proof.
+  (*** MS BEGIN {"type": "proof", "proof_type":"mirrorsolve", "total":2} *)
+  induction l;
+  prep_proof'.
+  - reflect insert_ordered_left_emp; 
+    check_goal_unsat.
+  - reflect insert_ordered_left_node; 
+    check_goal_unsat. 
+(*** MS END {"type": "proof", "proof_type":"mirrorsolve", "total":2} *)
+Admitted.
+
+(*** MS BEGIN {"type": "configuration", "config_type":"boilerplate"} *)
+MetaCoq Quote Definition insert_ordered_right_emp := (
+  (forall (r : tree V) (k k' : Z) (v : V), (k' < k)%Z -> gt_t k' r -> gt_t k' (insert k v r)) ->
+(forall (l : tree V) (k k' : Z) (v : V), (k < k')%Z -> lt_t k' l -> lt_t k' (insert k v l)) ->
+(forall (d : V) (x : Z) (l : tree V) (y : Z) (v : V) (r : tree V),
+ lookup d x (Node l y v r) = ite (x <? y)%Z (lookup d x l) (ite (x >? y)%Z (lookup d x r) v)) ->
+(forall (d : V) (x : Z), lookup d x Emp = d) ->
+(forall (x : Z) (l : tree V) (y : Z) (v : V) (r : tree V),
+ bound x (Node l y v r) = ite (x <? y)%Z (bound x l) (ite (x >? y)%Z (bound x r) true)) ->
+(forall x : Z, bound x Emp = false) ->
+(forall (x : Z) (v : V) (l : tree V) (y : Z) (v' : V) (r : tree V),
+ insert x v (Node l y v' r) =
+ ite (x <? y)%Z (Node (insert x v l) y v' r) (ite (x >? y)%Z (Node l y v' (insert x v r)) (Node l x v r))) ->
+(forall (x : Z) (v : V), insert x v Emp = Node Emp x v Emp) ->
+(forall (l : tree V) (k : Z) (v : V) (r : tree V),
+ (lt_t k l /\ gt_t k r /\ ordered l /\ ordered r -> ordered (Node l k v r)) /\
+ (ordered (Node l k v r) -> lt_t k l /\ gt_t k r /\ ordered l /\ ordered r)) ->
+ordered Emp ->
+(forall (k : Z) (l : tree V) (k' : Z) (v : V) (r : tree V),
+ ((k' > k)%Z /\ gt_t k l /\ gt_t k r -> gt_t k (Node l k' v r)) /\
+ (gt_t k (Node l k' v r) -> (k' > k)%Z /\ gt_t k l /\ gt_t k r)) ->
+(forall k : Z, gt_t k Emp) ->
+(forall (k : Z) (l : tree V) (k' : Z) (v : V) (r : tree V),
+ ((k' < k)%Z /\ lt_t k l /\ lt_t k r -> lt_t k (Node l k' v r)) /\
+ (lt_t k (Node l k' v r) -> (k' < k)%Z /\ lt_t k l /\ lt_t k r)) ->
+(forall k : Z, lt_t k Emp) ->
+forall (k k' : Z) (v : V), (k > k')%Z -> gt_t k' Emp -> ordered Emp -> ordered (insert k v Emp)
+).
+
+MetaCoq Quote Definition insert_ordered_right_node := (
+  forall (r1 : tree V) (k : Z) (v : V) (r2 : tree V),
+(forall (k0 k' : Z) (v0 : V), (k0 > k')%Z -> gt_t k' r1 -> ordered r1 -> ordered (insert k0 v0 r1)) ->
+(forall (k0 k' : Z) (v0 : V), (k0 > k')%Z -> gt_t k' r2 -> ordered r2 -> ordered (insert k0 v0 r2)) ->
+(forall (r : tree V) (k0 k' : Z) (v0 : V), (k' < k0)%Z -> gt_t k' r -> gt_t k' (insert k0 v0 r)) ->
+(forall (l : tree V) (k0 k' : Z) (v0 : V), (k0 < k')%Z -> lt_t k' l -> lt_t k' (insert k0 v0 l)) ->
+(forall (d : V) (x : Z) (l : tree V) (y : Z) (v0 : V) (r : tree V),
+ lookup d x (Node l y v0 r) = ite (x <? y)%Z (lookup d x l) (ite (x >? y)%Z (lookup d x r) v0)) ->
+(forall (d : V) (x : Z), lookup d x Emp = d) ->
+(forall (x : Z) (l : tree V) (y : Z) (v0 : V) (r : tree V),
+ bound x (Node l y v0 r) = ite (x <? y)%Z (bound x l) (ite (x >? y)%Z (bound x r) true)) ->
+(forall x : Z, bound x Emp = false) ->
+(forall (x : Z) (v0 : V) (l : tree V) (y : Z) (v' : V) (r : tree V),
+ insert x v0 (Node l y v' r) =
+ ite (x <? y)%Z (Node (insert x v0 l) y v' r) (ite (x >? y)%Z (Node l y v' (insert x v0 r)) (Node l x v0 r))) ->
+(forall (x : Z) (v0 : V), insert x v0 Emp = Node Emp x v0 Emp) ->
+(forall (l : tree V) (k0 : Z) (v0 : V) (r : tree V),
+ (lt_t k0 l /\ gt_t k0 r /\ ordered l /\ ordered r -> ordered (Node l k0 v0 r)) /\
+ (ordered (Node l k0 v0 r) -> lt_t k0 l /\ gt_t k0 r /\ ordered l /\ ordered r)) ->
+ordered Emp ->
+(forall (k0 : Z) (l : tree V) (k' : Z) (v0 : V) (r : tree V),
+ ((k' > k0)%Z /\ gt_t k0 l /\ gt_t k0 r -> gt_t k0 (Node l k' v0 r)) /\
+ (gt_t k0 (Node l k' v0 r) -> (k' > k0)%Z /\ gt_t k0 l /\ gt_t k0 r)) ->
+(forall k0 : Z, gt_t k0 Emp) ->
+(forall (k0 : Z) (l : tree V) (k' : Z) (v0 : V) (r : tree V),
+ ((k' < k0)%Z /\ lt_t k0 l /\ lt_t k0 r -> lt_t k0 (Node l k' v0 r)) /\
+ (lt_t k0 (Node l k' v0 r) -> (k' < k0)%Z /\ lt_t k0 l /\ lt_t k0 r)) ->
+(forall k0 : Z, lt_t k0 Emp) ->
+forall (k0 k' : Z) (v0 : V),
+(k0 > k')%Z -> gt_t k' (Node r1 k v r2) -> ordered (Node r1 k v r2) -> ordered (insert k0 v0 (Node r1 k v r2))
+).
+(*** MS END {"type": "configuration", "config_type":"boilerplate"} *)
+
+(*** MS BEGIN {"type": "proof_definition"} *)
+Lemma insert_ordered_right :
+forall (r: tree V) k k' v, 
+  (k > k')%Z -> 
+  gt_t k' r -> 
+  ordered r ->
+  ordered (insert k v r).
+(*** MS END {"type": "proof_definition"} *)
+Proof.
+  (*** MS BEGIN {"type": "proof", "proof_type":"manual"} *)
+  induction r;
+  intros;
+  simpl in *.
+  - intuition.
+  - destruct (k0 <? k)%Z eqn:?;
+    simpl in *.
+    * intuition.
+      eapply insert_left_lt;
+      eauto.
+      Lia.lia.
+    * destruct (k0 >? k)%Z eqn:?;
+      simpl in *; 
+      intuition.
+      + eapply insert_right_lt;
+        intuition.
+      + assert (k0 = k) by Lia.lia.
+        subst.
+        trivial.
+      + assert (k0 = k) by Lia.lia.
+        subst.
+        trivial.
+  Restart.
+  (*** MS END {"type": "proof", "proof_type":"manual"} *)
+Proof.
+  (*** MS BEGIN {"type": "proof", "proof_type":"hammer", "total":2, "finished":1} *)
+  induction r.
+  - hammer.
+  - admit. (* hammer. *)
+(*** MS END {"type": "proof", "proof_type":"hammer", "total":2, "finished":1} *)
+  Restart.
+Proof.
+  (*** MS BEGIN {"type": "proof", "proof_type":"mirrorsolve", "total":2} *)
+  induction r;
+  prep_proof'.
+  - reflect insert_ordered_right_emp; 
+    check_goal_unsat.
+  - reflect insert_ordered_right_node; 
+    check_goal_unsat.
+(*** MS END {"type": "proof", "proof_type":"mirrorsolve", "total":2} *)
+Admitted.
+  
+(*** MS BEGIN {"type": "configuration", "config_type":"tactics"} *)
+Ltac prep_proof'' := Utils.pose_all (tt, insert_ordered_left, insert_ordered_right);
+  prep_proof'.
+(*** MS END {"type": "configuration", "config_type":"tactics"} *)
+
+(*** MS BEGIN {"type": "configuration", "config_type":"boilerplate"} *)
+MetaCoq Quote Definition insert_ordered_emp := (
+  
+(forall (r : tree V) (k k' : Z) (v : V), (k > k')%Z -> gt_t k' r -> ordered r -> ordered (insert k v r)) ->
+(forall (l : tree V) (k k' : Z) (v : V), (k < k')%Z -> lt_t k' l -> ordered l -> ordered (insert k v l)) ->
+(forall (r : tree V) (k k' : Z) (v : V), (k' < k)%Z -> gt_t k' r -> gt_t k' (insert k v r)) ->
+(forall (l : tree V) (k k' : Z) (v : V), (k < k')%Z -> lt_t k' l -> lt_t k' (insert k v l)) ->
+(forall (d : V) (x : Z) (l : tree V) (y : Z) (v : V) (r : tree V),
+ lookup d x (Node l y v r) = ite (x <? y)%Z (lookup d x l) (ite (x >? y)%Z (lookup d x r) v)) ->
+(forall (d : V) (x : Z), lookup d x Emp = d) ->
+(forall (x : Z) (l : tree V) (y : Z) (v : V) (r : tree V),
+ bound x (Node l y v r) = ite (x <? y)%Z (bound x l) (ite (x >? y)%Z (bound x r) true)) ->
+(forall x : Z, bound x Emp = false) ->
+(forall (x : Z) (v : V) (l : tree V) (y : Z) (v' : V) (r : tree V),
+ insert x v (Node l y v' r) =
+ ite (x <? y)%Z (Node (insert x v l) y v' r) (ite (x >? y)%Z (Node l y v' (insert x v r)) (Node l x v r))) ->
+(forall (x : Z) (v : V), insert x v Emp = Node Emp x v Emp) ->
+(forall (l : tree V) (k : Z) (v : V) (r : tree V),
+ (lt_t k l /\ gt_t k r /\ ordered l /\ ordered r -> ordered (Node l k v r)) /\
+ (ordered (Node l k v r) -> lt_t k l /\ gt_t k r /\ ordered l /\ ordered r)) ->
+ordered Emp ->
+(forall (k : Z) (l : tree V) (k' : Z) (v : V) (r : tree V),
+ ((k' > k)%Z /\ gt_t k l /\ gt_t k r -> gt_t k (Node l k' v r)) /\
+ (gt_t k (Node l k' v r) -> (k' > k)%Z /\ gt_t k l /\ gt_t k r)) ->
+(forall k : Z, gt_t k Emp) ->
+(forall (k : Z) (l : tree V) (k' : Z) (v : V) (r : tree V),
+ ((k' < k)%Z /\ lt_t k l /\ lt_t k r -> lt_t k (Node l k' v r)) /\
+ (lt_t k (Node l k' v r) -> (k' < k)%Z /\ lt_t k l /\ lt_t k r)) ->
+(forall k : Z, lt_t k Emp) -> forall (k : Z) (v : V), ordered Emp -> ordered (insert k v Emp)
+).
+
+MetaCoq Quote Definition insert_ordered_node := (
+  forall (t1 : tree V) (k : Z) (v : V) (t2 : tree V),
+(forall (k0 : Z) (v0 : V), ordered t1 -> ordered (insert k0 v0 t1)) ->
+(forall (k0 : Z) (v0 : V), ordered t2 -> ordered (insert k0 v0 t2)) ->
+(forall (r : tree V) (k0 k' : Z) (v0 : V), (k0 > k')%Z -> gt_t k' r -> ordered r -> ordered (insert k0 v0 r)) ->
+(forall (l : tree V) (k0 k' : Z) (v0 : V), (k0 < k')%Z -> lt_t k' l -> ordered l -> ordered (insert k0 v0 l)) ->
+(forall (r : tree V) (k0 k' : Z) (v0 : V), (k' < k0)%Z -> gt_t k' r -> gt_t k' (insert k0 v0 r)) ->
+(forall (l : tree V) (k0 k' : Z) (v0 : V), (k0 < k')%Z -> lt_t k' l -> lt_t k' (insert k0 v0 l)) ->
+(forall (d : V) (x : Z) (l : tree V) (y : Z) (v0 : V) (r : tree V),
+ lookup d x (Node l y v0 r) = ite (x <? y)%Z (lookup d x l) (ite (x >? y)%Z (lookup d x r) v0)) ->
+(forall (d : V) (x : Z), lookup d x Emp = d) ->
+(forall (x : Z) (l : tree V) (y : Z) (v0 : V) (r : tree V),
+ bound x (Node l y v0 r) = ite (x <? y)%Z (bound x l) (ite (x >? y)%Z (bound x r) true)) ->
+(forall x : Z, bound x Emp = false) ->
+(forall (x : Z) (v0 : V) (l : tree V) (y : Z) (v' : V) (r : tree V),
+ insert x v0 (Node l y v' r) =
+ ite (x <? y)%Z (Node (insert x v0 l) y v' r) (ite (x >? y)%Z (Node l y v' (insert x v0 r)) (Node l x v0 r))) ->
+(forall (x : Z) (v0 : V), insert x v0 Emp = Node Emp x v0 Emp) ->
+(forall (l : tree V) (k0 : Z) (v0 : V) (r : tree V),
+ (lt_t k0 l /\ gt_t k0 r /\ ordered l /\ ordered r -> ordered (Node l k0 v0 r)) /\
+ (ordered (Node l k0 v0 r) -> lt_t k0 l /\ gt_t k0 r /\ ordered l /\ ordered r)) ->
+ordered Emp ->
+(forall (k0 : Z) (l : tree V) (k' : Z) (v0 : V) (r : tree V),
+ ((k' > k0)%Z /\ gt_t k0 l /\ gt_t k0 r -> gt_t k0 (Node l k' v0 r)) /\
+ (gt_t k0 (Node l k' v0 r) -> (k' > k0)%Z /\ gt_t k0 l /\ gt_t k0 r)) ->
+(forall k0 : Z, gt_t k0 Emp) ->
+(forall (k0 : Z) (l : tree V) (k' : Z) (v0 : V) (r : tree V),
+ ((k' < k0)%Z /\ lt_t k0 l /\ lt_t k0 r -> lt_t k0 (Node l k' v0 r)) /\
+ (lt_t k0 (Node l k' v0 r) -> (k' < k0)%Z /\ lt_t k0 l /\ lt_t k0 r)) ->
+(forall k0 : Z, lt_t k0 Emp) ->
+forall (k0 : Z) (v0 : V), ordered (Node t1 k v t2) -> ordered (insert k0 v0 (Node t1 k v t2))
+).
+(*** MS END {"type": "configuration", "config_type":"boilerplate"} *)
+
+(*** MS BEGIN {"type": "proof_definition"} *)
+Theorem insert_ordered : 
+forall (t: tree V) k v,
+  ordered t -> 
+  ordered (insert k v t).
+(*** MS END {"type": "proof_definition"} *)
+Proof.
+  (*** MS BEGIN {"type": "proof", "proof_type":"manual"} *)
+  induction t;
+  intros;
+  simpl in *.
+  - intuition.
+  - destruct (k0 <? k)%Z eqn:?;
+    simpl in *.
+    * intuition.
+      eapply insert_left_lt;
+      intuition.
+    * destruct (k0 >? k)%Z eqn:?;
+      simpl in *; 
+      intuition.
+      + eapply insert_right_lt;
+        intuition.
+      + assert (k0 = k) by Lia.lia.
+        subst.
+        trivial.
+      + assert (k0 = k) by Lia.lia.
+        subst.
+        trivial.
+(*** MS END {"type": "proof", "proof_type":"manual"} *)
+  Restart.
+Proof.
+  (*** MS BEGIN {"type": "proof", "proof_type":"hammer", "total":2, "finished":1} *)
+  induction t.
+  - hammer.
+  - admit. (* hammer. *)
+(*** MS END {"type": "proof", "proof_type":"hammer", "total":2, "finished":1} *)
+  Restart.
+Proof.
+  (*** MS BEGIN {"type": "proof", "proof_type":"mirrorsolve", "total":2} *)
+  induction t;
+  prep_proof''.
+  - reflect insert_ordered_emp; 
+    check_goal_unsat.
+  - reflect insert_ordered_node; 
+    check_goal_unsat.
+(*** MS END {"type": "proof", "proof_type":"mirrorsolve", "total":2} *)
+Admitted.
